enhance: memory/thread-safe quasi-zero-cost API with tests

Cvc/Defs.lean
@@ -1,1209 +1,1202 @@
 /-
-Copyright (c) 2023-2025 by the authors listed in the file AUTHORS and their
+Copyright (c) 2025 by the authors listed in the file AUTHORS and their
 institutional affiliations. All rights reserved.
 Released under Apache 2.0 license as described in the file LICENSE.
 Authors: Adrien Champion
 -/
 
-import Cvc.Logic
-import Cvc.Basic
-import Cvc.Srt
-import Cvc.Option
+import Lean.Parser
+
+import Std.Data.HashMap.Basic
+
+import Cvc.Basic.Batteries
+import Cvc.Basic.Logic
+import Cvc.Basic.Srt
+import Cvc.Basic.Error
 
 
 
-/-! # Functions and monads for term, term building, SMT *etc.* helpers and monads -/
-namespace Cvc
+namespace Cvc open cvc5 renaming TermManager → Tm
 
 
 
-/-- Type-safe cvc5 terms, input type expected to be `IsSrt` for most uses.
-
-- No direct constructor exposed publicly, users must go through the `Term.Build` monadic
-  constructors.
--/
-structure Term (α : Type) where
-/-- Constructor from an unsafe term. -/
-private ofUnsafe ::
-  /-- True if the term mentions symbols. -/
-  hasSymbols : Bool
-  /-- Underlying unsafe term. -/
-  toUnsafe : cvc5.Term
-
-/-- Abbreviation for a `Term Bool`. -/
-abbrev Formula := Term Bool
+/-! ## Environment: `EnvT`, `Env` -/
 
 
 
-namespace Term
+protected class Scope : Prop where
+/-- Private constructor. -/
+private ofUnit ::
+  /-- Private projection to an irrelevant proof, never used. -/
+  private toUnit : True
 
-/-- Boolean terms: `Term Bool`. -/
-protected abbrev Bool := Term Bool
-/-- Integer terms: `Term Int`. -/
-protected abbrev Int := Term Int
-/-- Real/`Rat` terms: `Term Rat`. -/
-protected abbrev Real := Term Rat
-/-- String terms: `Term String`. -/
-protected abbrev String := Term String
-/-- Array terms. -/
-protected abbrev Array (α β : Type) := Term (Cvc.TMap α β)
-/-- Sequence terms. -/
-protected abbrev Seq (α : Type) := Term (Array α)
-/-- Function terms. -/
-protected abbrev Fun (α β : Type) := Term (α → β)
-/-- Product terms. -/
-protected abbrev Prod (α β : Type) := Term (α × β)
+namespace Scope
+
+def Stx.ident := ``Cvc.Scope |> Lean.mkIdent
+
+end Scope
 
 
 
-section variable [A : IsSrt α] (term : Term α)
-
-/-- Sort of some term.
-
-> Note that due to strong-typing, this function does not perform any FFI.
--/
-abbrev srt : (term : Term α) → Srt := 𝕂 A.srt
-
-theorem srt_bij : α = term.srt := A.h_bij
-
-/-- Re-types `t` in terms of the type of `t.srt`. -/
-def retype : Term term.srt := term.srt_bij ▸ term
-
-/-- Helper for dependent-pattern-matching the sort of a term. -/
-def inspectSrt (f : (srt : Srt) → Term srt → β) : β :=
-  f term.srt term.retype
-
-end
-
-
-
-/-- Monadic constructor from an unsafe term. -/
-private def ofUnsafeM [Monad m] [IsSrt α] (hasSymbols : Bool) : m cvc5.Term → m (Term α) :=
-  (Term.ofUnsafe hasSymbols <$> ·)
-
-/-- SMT-LIB string representation. -/
-def toSmtString (term : Term α) : String :=
-  term.toUnsafe.toString
-
-instance : ToString (Term α) := ⟨Term.toSmtString⟩
-
-
-
-/-! ## Term building -/
-open cvc5 renaming TermManager → Manager
-
-/-- State of the term builder monad. -/
-structure Build.State where
+/-- State of the environment monad. -/
+structure Env.State [Cvc.Scope] : Type where
 /-- Constructor from a term manager. -/
-mk' ::
-  /-- Term manager. -/
-  manager : Manager
+private mk ::
+  /-- `cvc5`'s term manager. -/
+  private manager : Tm
   /-- Logic builder, used to track the logic necessary to express the terms actually built.
 
   Updated when building terms.
   -/
-  logic : Logic.Builder := Logic.Builder.mk
+  private logic : Logic.Builder := Logic.Builder.mk
 
-namespace Build.State
+namespace Env.State
 
-@[inherit_doc Build.State.mk']
-def ofManager (manager : Manager) (logic : Logic.Builder := Logic.Builder.mk) : Build.State :=
-  ⟨manager, logic⟩
+/-- Creates a new environment state. -/
+private def new [Cvc.Scope] : cvc5.Env State := ({manager := ·}) <$> cvc5.TermManager.new
 
-/-- Creates a new term builder state. -/
-def mk : BaseIO Build.State :=
-  ofManager <$> cvc5.TermManager.new
+/-- Creates a new environment state for a specific scope. -/
+private def newIn (S : Cvc.Scope) : cvc5.Env State := new
 
-
-end Build.State
+end Env.State
 
 
 
-/-- Term-building error-state-monad transformer. -/
-abbrev BuildT (m : Type → Type u) :=
-  ResT (StateT Build.State m)
+/-- Cvc environment monad transformer.
 
-/-- Term-building error-state-monad in `IO`. -/
-abbrev BuildIO := BuildT IO
+It should almost always be the case that `MonadLiftT BaseIO m`.
+-/
+def EnvT [Cvc.Scope] (m : Type → Type) (α : Type) : Type :=
+  Env.State → m (Except Error α × Env.State)
 
-/-- Plain term-building error-state-monad. -/
-abbrev Build := BuildT Id
+/-- Cvc environment monad, in `BaseIO`.
 
-namespace BuildT
+This monad is compatible with `IO`.
+-/
+abbrev Env [Cvc.Scope] (α : Type) : Type :=
+  EnvT BaseIO α
 
-example [Monad m] : MonadLiftT Res (BuildT m) := inferInstance
+namespace EnvT
 
-instance : MonadLift (Except cvc5.Error) Build where
-  monadLift code tm := do
-    match ← code with
-    | .ok res => return (.ok res, tm)
-    | .error error => return (.error <| Error.ofCvc5 error, tm)
+instance [Cvc.Scope] [Monad m] : Monad (EnvT m) where
+  pure a state := return (.ok a, state)
+  bind a f state := do
+    match ← a state with
+    | (.ok a, state) => f a state
+    | (.error e, state) => return (.error e, state)
 
-instance [Monad m] : MonadLift Build (BuildT m) :=
-  ⟨fun code state => return code state⟩
+instance [Cvc.Scope] [Monad m] [MonadLiftT BaseIO m] : MonadLift Env (EnvT m) where
+  monadLift code state := do
+    let res ← code state
+    return res
 
-instance [Monad m] [MonadLiftT IO m] : MonadLift BuildIO (BuildT m) :=
-  ⟨fun code state => return ← code state⟩
+instance [Cvc.Scope] [Monad m] : MonadLift m (EnvT m) where
+  monadLift mCode state := return (← .ok <$> mCode, state)
 
-/-- Runs term-building code with a specific build state. -/
-def runWith' (build : BuildT m α) (state : Build.State) : m (Except Error α × Build.State) :=
-  build state
+instance [Cvc.Scope] [Monad m] : MonadLift (Except Error) (EnvT m) where
+  monadLift exc state := return (exc, state)
 
-section variable [Monad m]
+instance [Cvc.Scope] [Monad m] : MonadLift (ExceptT Error m) (EnvT m) where
+  monadLift exc state := return (← exc, state)
 
-@[inherit_doc runWith']
-def runWith (build : BuildT m α) (state : Build.State) : m (Except Error α) :=
-  Prod.fst <$> build.runWith' state
+instance [Cvc.Scope] [Monad m] : MonadState Env.State (EnvT m) where
+  get state := return (.ok state, state)
+  set state _state := return (.ok (), state)
+  modifyGet f state :=
+    let (res, state) := f state
+    return (.ok res, state)
 
-section variable [MonadLiftT BaseIO m]
+instance [Cvc.Scope] [Monad m] : MonadExcept Error (EnvT m) where
+  throw e state := return (.error e, state)
+  tryCatch code errorDo state := do
+    match ← code state with
+    | pair@(.ok _, _) => return pair
+    | (.error e, state) => errorDo e state
 
-/-- Runs term-building code, creates an initial build state if none is provided. -/
-def run' [MonadLiftT BaseIO m]
-  (build : BuildT m α) (state? : Option Build.State := none)
-: m (Except Error α × Build.State) := do
-  let state ← if let some state := state? then pure state else Build.State.mk
-  build state
+instance [Cvc.Scope] [Monad m] [MonadLiftT BaseIO m] : MonadLift IO (EnvT m) where
+  monadLift ioCode state := do
+    match ← ioCode.toBaseIO with
+    | .ok a => return (.ok a, state)
+    | .error e => return (toString e |> .io |> .error, state)
 
-@[inherit_doc run']
-def run [MonadLiftT BaseIO m]
-  (build : BuildT m α) (state? : Option Build.State := none)
-: m (Except Error α) :=
-  Prod.fst <$> build.run' state?
+private instance [Cvc.Scope] [Monad m] : MonadLift (cvc5.EnvT m) (EnvT m) where
+  monadLift unsafeCode state :=
+    return ((← unsafeCode).mapError Error.ofUnsafe, state)
+
+/-- Runs `EnvT` code. -/
+def run [Monad m] [MonadLiftT BaseIO m]
+  (code : [Cvc.Scope] → EnvT m α)
+: m (Except Error α) := do
+  let S : Cvc.Scope := ⟨True.intro⟩
+  match ← Env.State.newIn S |>.run with
+  | .ok state => Prod.fst <$> code state
+  | .error e => return .error e
+
+end EnvT
+
+
+
+namespace Env variable [Cvc.Scope]
+
+def Stx.ident := ``Env |> Lean.mkIdent
+
+-- sanity
+example : Monad Env := inferInstance
+example : MonadLift BaseIO Env := inferInstance
+example : MonadLift (Except Error) Env := inferInstance
+example : MonadLift (ExceptT Error BaseIO) Env := inferInstance
+example : MonadState Env.State Env := inferInstance
+example : MonadExcept Error Env := inferInstance
+example : MonadLift IO Env := inferInstance
+example : MonadLift cvc5.Env Env := inferInstance
+
+/-- Runs `Env` code. -/
+def run (code : [Cvc.Scope] → Env α) : BaseIO (Except Error α) :=
+  EnvT.run code
+
+/-- Runs `Env` code in `IO`. -/
+def runIO (code : [Cvc.Scope] → Env α) : IO α := do
+  match ←run code with
+  | .ok a => return a
+  | .error e => throw <| IO.userError <| toString e
+
+end Env
+
+
+
+/-- Unsafe term manager accessor. -/
+private def getTm [Cvc.Scope] [Monad m] : EnvT m Tm :=
+  fun state => return (.ok state.manager, state)
+
+/-- Runs `cvc5.Env` code given the environment's underlying term manager. -/
+private def tmDoM [Cvc.Scope] [Monad m] (f : Tm → cvc5.EnvT m α) : EnvT m α :=
+  getTm >>= (liftM ∘ f)
+
+@[inherit_doc tmDoM]
+private def tmDo [Cvc.Scope] [Monad m] (f : Tm → α) : EnvT m α :=
+  tmDoM (pure ∘ f)
+
+
+
+/-! ## Sorts -/
+
+
+/-- Safe cvc5 sorts. -/
+def Srt [Cvc.Scope] := cvc5.Sort
+
+namespace Srt variable [Cvc.Scope]
+
+def Stx.ident := ``Srt |> Lean.mkIdent
+
+@[inherit_doc Tm.getBooleanSort]
+def bool : Env Srt := tmDoM Tm.getBooleanSort
+@[inherit_doc Tm.getIntegerSort]
+def int : Env Srt := tmDoM Tm.getIntegerSort
+@[inherit_doc Tm.getRealSort]
+def real : Env Srt := tmDoM Tm.getRealSort
+@[inherit_doc Tm.getRegExpSort]
+def regex : Env Srt := tmDoM Tm.getRegExpSort
+@[inherit_doc Tm.getRoundingModeSort]
+def roundingMode : Env Srt := tmDoM Tm.getRoundingModeSort
+@[inherit_doc Tm.getStringSort]
+def string : Env Srt := tmDoM Tm.getStringSort
+
+@[inherit_doc Tm.mkArraySort]
+def array (idx elm : Srt) : Env Srt :=
+  tmDoM fun tm => tm.mkArraySort idx elm
+
+@[inherit_doc Tm.mkBitVectorSort]
+def bitVec (size : UInt32) : Env Srt :=
+  tmDoM fun tm => tm.mkBitVectorSort size
+
+@[inherit_doc Tm.mkFloatingPointSort]
+def float (exp sig : UInt32) : Env Srt :=
+  tmDoM fun tm => tm.mkFloatingPointSort exp sig
+
+@[inherit_doc Tm.mkFiniteFieldSort]
+def finiteField (size : Nat) (base : UInt32 := 10) : Env Srt :=
+  tmDoM fun tm => tm.mkFiniteFieldSort size base
+
+@[inherit_doc Tm.mkFunctionSort]
+def function (dom : Array Srt) (cod : Srt) : Env Srt :=
+  tmDoM fun tm => tm.mkFunctionSort dom cod
+
+@[inherit_doc Tm.mkPredicateSort]
+def predicate (dom : Array Srt) : Env Srt :=
+  tmDoM fun tm => tm.mkPredicateSort dom
+
+@[inherit_doc Tm.mkTupleSort]
+def tuple (dom : Array Srt) : Env Srt :=
+  tmDoM fun tm => tm.mkTupleSort dom
+
+@[inherit_doc Tm.mkUninterpretedSortConstructorSort]
+def uninterpretedSortConstructor (arity : Nat) (symbol : String) : Env Srt :=
+  tmDoM fun tm => tm.mkUninterpretedSortConstructorSort arity symbol
+
+@[inherit_doc Tm.mkSetSort]
+def set (sort : Srt) : Env Srt :=
+  tmDoM fun tm => tm.mkSetSort sort
+@[inherit_doc Tm.mkBagSort]
+def bag (sort : Srt) : Env Srt :=
+  tmDoM fun tm => tm.mkBagSort sort
+@[inherit_doc Tm.mkSequenceSort]
+def seq (sort : Srt) : Env Srt :=
+  tmDoM fun tm => tm.mkSequenceSort sort
+
+@[inherit_doc Tm.mkAbstractSort]
+def abstract (kind : Srt.Kind) : Env Srt :=
+  tmDoM fun tm => tm.mkAbstractSort kind
+
+@[inherit_doc Tm.mkUninterpretedSort]
+def uninterpreted (symbol : String) : Env Srt :=
+  tmDoM fun tm => tm.mkUninterpretedSort symbol
+
+@[inherit_doc Tm.mkNullableSort]
+def nullable (sort : Srt) : Env Srt :=
+  tmDoM fun tm => tm.mkNullableSort sort
+
+@[inherit_doc Tm.mkParamSort]
+def param (symbol : String) : Env Srt :=
+  tmDoM fun tm => tm.mkParamSort symbol
+
+
+
+/-- Constructor from an unsafe `cvc5` sort. -/
+private def ofUnsafe (sort : cvc5.Sort) : Srt := sort
+
+section variable (sort : Srt)
+
+/-- Unsafe `cvc5` version of an `Srt`. -/
+private def toUnsafe : cvc5.Sort := sort
+
+@[inherit_doc cvc5.Sort.getKind]
+def getKind : Env Srt.Kind := sort.toUnsafe.getKind |> Kind.ofUnsafe |> pure
+
+@[inherit_doc getKind]
+def Kind.ofSrt := sort.getKind
+
+@[inherit_doc cvc5.Sort.isBoolean]
+def isBool : Env Bool := return sort.toUnsafe.isBoolean
+@[inherit_doc cvc5.Sort.isInteger]
+def isInt : Env Bool := return sort.toUnsafe.isInteger
+@[inherit_doc cvc5.Sort.isReal]
+def isReal : Env Bool := return sort.toUnsafe.isReal
+@[inherit_doc cvc5.Sort.isString]
+def isString : Env Bool := return sort.toUnsafe.isString
+@[inherit_doc cvc5.Sort.isRegExp]
+def isRegexp : Env Bool := return sort.toUnsafe.isRegExp
+@[inherit_doc cvc5.Sort.isRoundingMode]
+def isRoundingMode : Env Bool := return sort.toUnsafe.isRoundingMode
+@[inherit_doc cvc5.Sort.isBitVector]
+def isBitVec : Env Bool := return sort.toUnsafe.isBitVector
+@[inherit_doc cvc5.Sort.isFloatingPoint]
+def isFloat : Env Bool := return sort.toUnsafe.isFloatingPoint
+@[inherit_doc cvc5.Sort.isDatatype]
+def isDatatype : Env Bool := return sort.toUnsafe.isDatatype
+@[inherit_doc cvc5.Sort.isDatatypeConstructor]
+def isDatatypeConstructor : Env Bool := return sort.toUnsafe.isDatatypeConstructor
+@[inherit_doc cvc5.Sort.isDatatypeSelector]
+def isDatatypeSelector : Env Bool := return sort.toUnsafe.isDatatypeSelector
+@[inherit_doc cvc5.Sort.isDatatypeTester]
+def isDatatypeTester : Env Bool := return sort.toUnsafe.isDatatypeTester
+@[inherit_doc cvc5.Sort.isDatatypeUpdater]
+def isDatatypeUpdater : Env Bool := return sort.toUnsafe.isDatatypeUpdater
+@[inherit_doc cvc5.Sort.isFunction]
+def isFunction : Env Bool := return sort.toUnsafe.isFunction
+@[inherit_doc cvc5.Sort.isPredicate]
+def isPredicate : Env Bool := return sort.toUnsafe.isPredicate
+@[inherit_doc cvc5.Sort.isTuple]
+def isTuple : Env Bool := return sort.toUnsafe.isTuple
+@[inherit_doc cvc5.Sort.isNullable]
+def isNullable : Env Bool := return sort.toUnsafe.isNullable
+@[inherit_doc cvc5.Sort.isRecord]
+def isRecord : Env Bool := return sort.toUnsafe.isRecord
+@[inherit_doc cvc5.Sort.isArray]
+def isArray : Env Bool := return sort.toUnsafe.isArray
+@[inherit_doc cvc5.Sort.isFiniteField]
+def isFiniteField : Env Bool := return sort.toUnsafe.isFiniteField
+@[inherit_doc cvc5.Sort.isSet]
+def isSet : Env Bool := return sort.toUnsafe.isSet
+@[inherit_doc cvc5.Sort.isBag]
+def isBag : Env Bool := return sort.toUnsafe.isBag
+@[inherit_doc cvc5.Sort.isSequence]
+def isSequence : Env Bool := return sort.toUnsafe.isSequence
+@[inherit_doc cvc5.Sort.isUninterpretedSort]
+def isUninterpreted : Env Bool := return sort.toUnsafe.isUninterpretedSort
+@[inherit_doc cvc5.Sort.isUninterpretedSortConstructor]
+def isUninterpretedSortConstructor : Env Bool :=
+  return sort.toUnsafe.isUninterpretedSortConstructor
+@[inherit_doc cvc5.Sort.isInstantiated]
+def isInstantiated : Env Bool := return sort.toUnsafe.isInstantiated
+
+@[inherit_doc cvc5.Sort.hasSymbol]
+def hasSymbol : Env Bool := sort.toUnsafe.hasSymbol
+
+@[inherit_doc cvc5.Sort.getSymbol]
+def getSymbol : Env String := sort.toUnsafe.getSymbol
+@[inherit_doc cvc5.Sort.getSymbol?]
+def getSymbol? : Env (Option String) := return sort.toUnsafe.getSymbol?
+
+@[inherit_doc cvc5.Sort.getFunctionArity]
+def getFunctionArity : Env Nat := sort.toUnsafe.getFunctionArity
+@[inherit_doc cvc5.Sort.getFunctionArity?]
+def getFunctionArity? : Env (Option Nat) := return sort.toUnsafe.getFunctionArity?
+
+@[inherit_doc cvc5.Sort.getFunctionDomainSorts]
+def getFunctionDomain : Env (Array Srt) :=
+  sort.toUnsafe.getFunctionDomainSorts
+@[inherit_doc cvc5.Sort.getFunctionDomainSorts?]
+def getFunctionDomain? : Env (Option (Array Srt)) :=
+  return sort.toUnsafe.getFunctionDomainSorts?
+
+@[inherit_doc cvc5.Sort.getFunctionCodomainSort]
+def getFunctionCodomain : Env Srt :=
+  sort.toUnsafe.getFunctionCodomainSort
+@[inherit_doc cvc5.Sort.getFunctionCodomainSort?]
+def getFunctionCodomain? : Env (Option Srt) :=
+  return sort.toUnsafe.getFunctionCodomainSort?
+
+@[inherit_doc cvc5.Sort.getArrayIndexSort]
+def getArrayIdx : Env Srt :=
+  sort.toUnsafe.getArrayIndexSort
+@[inherit_doc cvc5.Sort.getArrayIndexSort?]
+def getArrayIdx? : Env (Option Srt) :=
+  return sort.toUnsafe.getArrayIndexSort?
+
+@[inherit_doc cvc5.Sort.getArrayElementSort]
+def getArrayElm : Env Srt :=
+  sort.toUnsafe.getArrayElementSort
+@[inherit_doc cvc5.Sort.getArrayElementSort?]
+def getArrayElm? : Env (Option Srt) :=
+  return sort.toUnsafe.getArrayElementSort?
+
+@[inherit_doc cvc5.Sort.getSetElementSort]
+def getSetElm : Env Srt :=
+  sort.toUnsafe.getSetElementSort
+@[inherit_doc cvc5.Sort.getSetElementSort?]
+def getSetElm? : Env (Option Srt) :=
+  return sort.toUnsafe.getSetElementSort?
+
+@[inherit_doc cvc5.Sort.getBagElementSort]
+def getBagElm : Env Srt :=
+  sort.toUnsafe.getBagElementSort
+@[inherit_doc cvc5.Sort.getBagElementSort?]
+def getBagElm? : Env (Option Srt) :=
+  return sort.toUnsafe.getBagElementSort?
+
+@[inherit_doc cvc5.Sort.getSequenceElementSort]
+def getSeqElm : Env Srt :=
+  sort.toUnsafe.getSequenceElementSort
+@[inherit_doc cvc5.Sort.getSequenceElementSort?]
+def getSeqElm? : Env (Option Srt) :=
+  return sort.toUnsafe.getSequenceElementSort?
+
+@[inherit_doc cvc5.Sort.getAbstractedKind]
+def getAbstractedKind : Env Kind :=
+  sort.toUnsafe.getAbstractedKind
+@[inherit_doc cvc5.Sort.getAbstractedKind?]
+def getAbstractedKind? : Env (Option Kind) :=
+  return sort.toUnsafe.getAbstractedKind?.map .ofUnsafe
+
+@[inherit_doc cvc5.Sort.getUninterpretedSortConstructorArity]
+def getUninterpretedSortConstructorArity : Env UInt32 :=
+  sort.toUnsafe.getUninterpretedSortConstructorArity
+@[inherit_doc cvc5.Sort.getUninterpretedSortConstructorArity?]
+def getUninterpretedSortConstructorArity? : Env (Option UInt32) :=
+  return sort.toUnsafe.getUninterpretedSortConstructorArity?
+
+@[inherit_doc cvc5.Sort.getBitVectorSize]
+def getBitVecSize : Env UInt32 :=
+  sort.toUnsafe.getBitVectorSize
+@[inherit_doc cvc5.Sort.getBitVectorSize?]
+def getBitVecSize? : Env (Option UInt32) :=
+  return sort.toUnsafe.getBitVectorSize?
+
+@[inherit_doc cvc5.Sort.getFiniteFieldSize]
+def getFiniteFieldSizes : Env Nat :=
+  sort.toUnsafe.getFiniteFieldSize
+@[inherit_doc cvc5.Sort.getFiniteFieldSize?]
+def getFiniteFieldSize? : Env (Option Nat) :=
+  return sort.toUnsafe.getFiniteFieldSize?
+
+@[inherit_doc cvc5.Sort.getFloatingPointExponentSize]
+def getFloatingPointExponentSizes : Env UInt32 :=
+  sort.toUnsafe.getFloatingPointExponentSize
+@[inherit_doc cvc5.Sort.getFloatingPointExponentSize?]
+def getFloatingPointExponentSize? : Env (Option UInt32) :=
+  return sort.toUnsafe.getFloatingPointExponentSize?
+
+@[inherit_doc cvc5.Sort.getFloatingPointSignificandSize]
+def getFloatingPointSignificandSizes : Env UInt32 :=
+  sort.toUnsafe.getFloatingPointSignificandSize
+@[inherit_doc cvc5.Sort.getFloatingPointSignificandSize?]
+def getFloatingPointSignificandSize? : Env (Option UInt32) :=
+  return sort.toUnsafe.getFloatingPointSignificandSize?
+
+@[inherit_doc cvc5.Sort.getTupleLength]
+def getTupleLengths : Env UInt32 :=
+  sort.toUnsafe.getTupleLength
+@[inherit_doc cvc5.Sort.getTupleLength?]
+def getTupleLength? : Env (Option UInt32) :=
+  return sort.toUnsafe.getTupleLength?
+
+@[inherit_doc cvc5.Sort.getTupleSorts]
+def getTupleSorts : Env (Array Srt) :=
+  sort.toUnsafe.getTupleSorts
+@[inherit_doc cvc5.Sort.getTupleSorts?]
+def getTupleSorts? : Env (Option (Array Srt)) :=
+  return sort.toUnsafe.getTupleSorts?
+
+@[inherit_doc cvc5.Sort.getNullableElementSort]
+def getNullableElementSort : Env Srt :=
+  sort.toUnsafe.getNullableElementSort
+@[inherit_doc cvc5.Sort.getNullableElementSort?]
+def getNullableElementSort? : Env (Option Srt) :=
+  return sort.toUnsafe.getNullableElementSort?
+
+@[inherit_doc cvc5.Sort.getUninterpretedSortConstructor]
+def getUninterpretedSortConstructor : Env Srt :=
+  sort.toUnsafe.getUninterpretedSortConstructor
+@[inherit_doc cvc5.Sort.getUninterpretedSortConstructor?]
+def getUninterpretedSortConstructor? : Env (Option Srt) :=
+  return sort.toUnsafe.getUninterpretedSortConstructor?
+
+@[inherit_doc cvc5.Sort.getInstantiatedParameters]
+def getInstantiatedParameters : Env (Array Srt) :=
+  sort.toUnsafe.getInstantiatedParameters
+@[inherit_doc cvc5.Sort.getInstantiatedParameters?]
+def getInstantiatedParameters? : Env (Option (Array Srt)) :=
+  return sort.toUnsafe.getInstantiatedParameters?
+
+@[inherit_doc cvc5.Sort.instantiate]
+def instantiate (params : Array Srt) : Env Srt :=
+  sort.toUnsafe.instantiate (params.map toUnsafe)
+@[inherit_doc cvc5.Sort.instantiate?]
+def instantiate? (params : Array Srt) : Env (Option Srt) :=
+  return sort.toUnsafe.instantiate? params
+
+@[inherit_doc cvc5.Sort.substitute]
+def substituteMap (map : Array (Srt × Srt)) : Env Srt := do
+  let mut sorts := Array.mkEmpty map.size
+  let mut sorts' := Array.mkEmpty map.size
+  for (sort, sort') in map do
+    sorts := sorts.push sort
+    sorts' := sorts'.push sort'
+  sort.toUnsafe.substitute sorts sorts'
+@[inherit_doc cvc5.Sort.substitute]
+def substitute (src tgt : Array Srt) :
+  (h : src.size ≤ tgt.size := by (try simp) <;> grind) → Env Srt
+:= fun _ =>
+  let sorts := src.map toUnsafe
+  let sorts' := tgt.take sorts.size |>.map toUnsafe
+  sort.toUnsafe.substitute sorts sorts'
+
+
+
+@[inherit_doc cvc5.Sort.toString]
+protected def toSmtString : Env String :=
+  return sort.toUnsafe.toString
 
 end
-
-end
-
-/-- Runs term-building code in `IO`, creates an initial build state if none is provided -/
-def runIO'
-  (build : BuildIO α) (state? : Option Build.State := none)
-: IO (α × Build.State) := do
-  let (a?, state) ← build.run' state?
-  match a? with
-  | .ok a => return (a, state)
-  | .error error =>
-    IO.eprintln s!"{error}"
-    throw <| IO.Error.userError error.toString
-
-@[inherit_doc runIO']
-def runIO (build : BuildIO α) (state? : Option Build.State := none) : IO α :=
-  Prod.fst <$> build.runIO' state?
-
-end BuildT
-
--- export `BuildT.<run>` runners to `Build.<run>`
-namespace Build
-export BuildT (runWith' runWith run' run runIO' runIO)
-end Build
-
--- also export `Term.BuildT.<run>`/`Term.Build.<run>` runners to `Term.<run>`
-export Build (runWith' runWith run' run runIO' runIO)
-
-
-
-
-/-- Applies a monadic function to the term manager part of the `Build.State`. -/
-private def managerDoM [Monad m] [MonadLiftT m Build] (f : Manager → m γ) : Build γ := do
-  let state ← get
-  f state.manager
-
-/-- Applies a function to the term manager part of the `Build.State`. -/
-private def managerDo (f : Manager → γ) : Build γ :=
-  managerDoM (m := Id) f
-
-/-- Applies a function to the `Logic.Builder` part of the `Build.State`. -/
-private def logicDo (f : Logic.Builder → Logic.Builder) : Build Unit :=
-  fun state =>
-    let logic := f state.logic
-    return (.ok (), {state with logic})
-
-end Term
-
-
-
-namespace Srt
-
-
-/-- Conversion to unsafe sorts.
-
-- function sorts are flattened:\
-  `srt → srt' → srt'' → nonFunSrt` becomes `#[srt, srt', srt''] → nonFunSrt`
--/
-def toSort (srt : Srt) : Term.Build cvc5.Sort :=
-  Term.managerDoM fun tm => aux tm srt 10_000
-where
-  aux (tm : cvc5.TermManager) (srt' : Srt) : (maxRec : Nat) → Term.Build cvc5.Sort
-    | 0 => Cvc.throwInternal s!"[Srt.toSort] maximum depth reached on `{srt}`"
-    | maxRec + 1 =>
-      match srt' with
-      | .bool => pure tm.getBooleanSort
-      | .int => pure tm.getIntegerSort
-      | .real => pure tm.getRealSort
-      | .regex => pure tm.getRegExpSort
-      | .string => pure tm.getStringSort
-      | .roundingMode => pure tm.getRoundingModeSort
-      | .finiteField size => tm.mkFiniteFieldSort size
-      | .bitVec size => tm.mkBitVectorSort size
-      | .float exp sig => tm.mkFloatingPointSort exp sig
-      | .uninterpreted name => pure <| tm.mkUninterpretedSort name
-      | .bag elm => do tm.mkBagSort (← aux tm elm maxRec)
-      | .seq elm => do tm.mkSequenceSort (← aux tm elm maxRec)
-      | .set elm => do tm.mkSetSort (← aux tm elm maxRec)
-      | .array idx elm => do tm.mkArraySort (← aux tm idx maxRec) (← aux tm elm maxRec)
-      | .function dom cod => do
-        let (doms, cod) ← flattenFun tm maxRec #[← aux tm dom maxRec] cod
-        tm.mkFunctionSort doms cod
-      | .prod lft rgt => do tm.mkTupleSort #[← aux tm lft maxRec, ← aux tm rgt maxRec]
-      | .unit => tm.mkTupleSort #[]
-      | .abstract _k => Cvc.throwInternal s!"[Srt.toSort] todo `{srt'}`"
-  flattenFun (tm : cvc5.TermManager) (maxRec : Nat)
-    (doms : Array cvc5.Sort)
-  : (cod : Srt) → Term.Build (Array cvc5.Sort × cvc5.Sort)
-    | .function dom cod => do
-      let dom ← aux tm dom maxRec
-      flattenFun tm maxRec (doms.push dom) cod
-    | cod => return (doms, (← aux tm cod maxRec))
-
-/-- Retrieves the domain and codomain of `srt` for `declareFun`-like functions.
-
-This function uncurries `α → β → ... → γ` to `#[α, β, ...] → γ`.
--/
-private def toSignature! (srt : Srt) : Term.Build (Array cvc5.Sort × cvc5.Sort) :=
-  Term.managerDoM (toSort.flattenFun srt · 10_000 #[] srt)
 
 end Srt
 
 
 
-/-! ## Term creation API -/
-namespace Term
-
-/-- Unsafe term creation. -/
-private def mk [IsSrt α]
-  (hasSymbols : Bool) (k : cvc5.Kind) (args : Array cvc5.Term)
-: Build (Term α) :=
-  managerDoM fun tm => ofUnsafe hasSymbols <$> tm.mkTerm k args
-
-
-
-/-- Builds a constant Boolean term. -/
-def bool (b : Bool) : Build Term.Bool :=
-  managerDo fun tm => tm.mkBoolean b |> Term.ofUnsafe false
-
-/-- Retrieves the value of a constant Boolean term. -/
-def boolVal? (t : Term.Bool) : Option Bool :=
-  t.toUnsafe.getBooleanValue?
-
-@[inherit_doc boolVal?]
-def boolVal (t : Term.Bool) : Res Bool :=
-  if let some t := t.boolVal?
-  then return t
-  else
-    Res.failUser "cannot retrieve Boolean value of a non-constant term"
-    |>.context s!"on term `{t}`"
-
-/-- Builds a constant integer term. -/
-def int (i : Int) : Build Term.Int := do
-  logicDo .int
-  managerDo fun tm => tm.mkInteger i |> Term.ofUnsafe false
-
-/-- Retrieves the value of a constant integer term. -/
-def intVal? (t : Term.Int) : Option Int :=
-  t.toUnsafe.getIntegerValue?
-
-@[inherit_doc intVal?]
-def intVal (t : Term.Int) : Res Int :=
-  if let some t := t.intVal?
-  then return t
-  else
-    Res.failUser "cannot retrieve integer value of a non-constant term"
-    |>.context s!"on term `{t}`"
-
-/-- Retrieves the value of a constant rational/real term. -/
-def ratVal? (t : Term.Real) : Res (Option Rat) :=
-  t.toUnsafe.getRationalValue?.mapM fun r =>
-    if h : r.den ≠ 0 then return Rat.normalize r.num r.den h
-    else Res.failInternal s!"cvc5 produced an illegal ration value: `{r}`"
-
-@[inherit_doc ratVal?]
-def ratVal (t : Term.Real) : Res Rat := do
-  if let some r ← t.ratVal? then return r else
-    Res.failUser "cannot retrieve rational value of a non-constant term"
-    |>.context s!"on term `{t}`"
-
--- /-- Retrieves the value of a constant rational/real term. -/
--- def stringVal? (t : Term.String) : Option String :=
---   t.toUnsafe.getStringValue?
-
--- @[inherit_doc stringVal?]
--- def stringVal (t : Term.String) : Res String := do
---   if let some r ← t.stringVal? then return r else
---     Res.failUser "cannot retrieve string value of a non-constant term"
---     |>.context s!"on term `{t}`"
-
-/-- Builds the Boolean negation of a term. -/
-def mkNot (term : Term.Bool) : Build Term.Bool :=
-  mk term.hasSymbols .NOT #[term.toUnsafe]
-
-@[inherit_doc mkNot]
-def not := mkNot
-
-/-- Builds an if-then-else term. -/
-def ite [IsSrt α] (cnd : Term.Bool) (thn els : Term α) : Build (Term α) :=
-  mk (cnd.hasSymbols ∨ thn.hasSymbols ∨ els.hasSymbols)
-    .ITE #[cnd.toUnsafe, thn.toUnsafe, els.toUnsafe]
-
-
-
-/-! ### `n`-ary operators (`2 ≤ n`) -/
-section nary2_bool
-variable (terms : Array (Term Bool)) (lft rgt : Term Bool)
-variable (h_size : 2 ≤ terms.size := by
-  (try (try simp <;> try omega) ; done)
-  <;> fail "expected an array of **at least** two terms"
-)
-
-/-- Builds a conjunction term. -/
-def mkAnd : Build Formula :=
-  let _ := h_size
-  mk (terms.any hasSymbols) .AND (terms.map toUnsafe)
-
-@[inherit_doc mkAnd]
-def and : Build Formula :=
-  mkAnd #[lft, rgt]
-
--- def iand (k : Nat) (i j : Term Int) : Build Formula := do
---   sorry
-
-/-- Builds a disjunction term. -/
-def mkOr : Build Formula :=
-  let _ := h_size
-  mk (terms.any hasSymbols) .OR (terms.map toUnsafe)
+/-! ## Untyped terms -/
 
-@[inherit_doc mkOr]
-def or : Build Formula :=
-  mkOr #[lft, rgt]
 
-/-- Builds an exclusive-disjunction term. -/
-def mkXor : Build Formula :=
-  let _ := h_size
-  mk (terms.any hasSymbols) .XOR (terms.map toUnsafe)
 
-@[inherit_doc mkXor]
-def xor : Build Formula :=
-  mkXor #[lft, rgt]
+/-- Type-unsafe cvc5 terms. -/
+def Term [Cvc.Scope] : Type := cvc5.Term
 
-/-- Builds a disjunction term. -/
-def mkImplies : Build Formula :=
-  let _ := h_size
-  mk (terms.any hasSymbols) .IMPLIES (terms.map toUnsafe)
+/-- An array of terms. -/
+abbrev Terms [Cvc.Scope] : Type := Array Term
 
-@[inherit_doc mkImplies]
-def implies : Build Formula :=
-  mkImplies #[lft, rgt]
 
-end nary2_bool
 
+namespace Term variable [Cvc.Scope]
 
 
-section nary2_generic
-variable [IsSrt α] (terms : Array (Term α)) (lft rgt : Term α)
-variable (h_size : 2 ≤ terms.size := by
-  (try (try simp <;> try omega) ; done)
-  <;> fail "expected an array of **at least** two terms"
-)
-
-/-- Builds an equality term. -/
-def mkEqual : Build Formula :=
-  let _ := h_size
-  mk (terms.any hasSymbols) .EQUAL (terms.map toUnsafe)
-
-@[inherit_doc mkEqual]
-def equal : Build Formula :=
-  mkEqual #[lft, rgt]
-
-/-- Builds a pairwise-*distinct* term. -/
-def mkDistinct : Build Formula :=
-  let _ := h_size
-  mk (terms.any hasSymbols) .DISTINCT (terms.map toUnsafe)
-
-@[inherit_doc mkDistinct]
-def distinct : Build Formula :=
-  mkDistinct #[lft, rgt]
-
-@[inherit_doc mkDistinct]
-abbrev mkNEqual := @distinct
-@[inherit_doc distinct]
-abbrev nequal := @distinct
-
-end nary2_generic
-
-
-
-section nary2_arith
-variable [IsSrt.Arith α] (terms : Array (Term α)) (lft rgt : Term α)
-variable (h_size : 2 ≤ terms.size := by
-  (try (try simp <;> try omega) ; done)
-  <;> fail "expected an array of **at least** two terms"
-)
-
-/-- Builds a less-than term. -/
-def mkLt : Build Formula :=
-  let _ := h_size
-  mk (terms.any hasSymbols) .LT (terms.map toUnsafe)
-
-@[inherit_doc mkLt]
-def lt : Build Formula :=
-  mkLt #[lft, rgt]
-
-/-- Builds a less-than-or-equal-to term. -/
-def mkLe : Build Formula :=
-  let _ := h_size
-  mk (terms.any hasSymbols) .LEQ (terms.map toUnsafe)
-
-@[inherit_doc mkLe]
-def le : Build Formula :=
-  mkLe #[lft, rgt]
-
-/-- Builds a greater-than-or-equal-to term. -/
-def mkGe : Build Formula :=
-  let _ := h_size
-  mk (terms.any hasSymbols) .GEQ (terms.map toUnsafe)
-
-@[inherit_doc mkGe]
-def ge : Build Formula :=
-  mkGe #[lft, rgt]
-
-/-- Builds a greater-than term. -/
-def mkGt : Build Formula :=
-  let _ := h_size
-  mk (terms.any hasSymbols) .GT (terms.map toUnsafe)
-
-@[inherit_doc mkGt]
-def gt : Build Formula :=
-  mkGt #[lft, rgt]
-
-end nary2_arith
-
-
-
-/-! #### Arithmetic -/
-section arith
-
-variable [IsSrt α] (terms : Array (Term α)) (term lft rgt : Term α)
-variable (h_size : 2 ≤ terms.size := by
-  (try (try simp <;> try omega) ; done)
-  <;> fail "expected an array of **at least** two terms"
-)
-variable (Arith : IsSrt.Arith α := by
-  (try ( exact inferInstance ) ; done)
-  <;> fail "expected arithmetic type `Int` or `Rat`, see `Cvc.is_arith` and `Cvc.IsSrt.Arith`"
-)
-
-/-- Forbids difference logics. -/
-private def nonDiff : Build Unit := logicDo .nonDiff
-
-/-- Forces non-linear logic if non-linear, true if one of the terms has symbols. -/
-private def checkNonLinearOfArgs (terms : Array (Term α)) : Build Bool := do
-  let mut hasSymbols := false
-  let mut nonLinear := false
-  for term in terms do
-    if term.hasSymbols then
-      if hasSymbols then
-        nonLinear := true
-        break
-      else
-        hasSymbols := true
-  if nonLinear then
-    logicDo (.nonLinear ∘ .nonDiff)
-  return hasSymbols
-
-/-- Builds an addition term.
-
-- Forbids difference logics.
--/
-def mkAdd : Build (Term α) := do
-  nonDiff
-  let _ := h_size ; let _ := Arith
-  mk (terms.any hasSymbols) .ADD (terms.map toUnsafe)
-
-@[inherit_doc mkAdd]
-def add : Build (Term α) :=
-  mkAdd #[lft, rgt]
-
-/-- Builds a subtraction term. -/
-def mkSub : Build (Term α) := do
-  nonDiff
-  let _ := h_size ; let _ := Arith
-  mk (terms.any hasSymbols) .SUB (terms.map toUnsafe)
-
-@[inherit_doc mkSub]
-def sub : Build (Term α) :=
-  mkSub #[lft, rgt]
-
-def neg : Build (Term α) :=
-  let _ := Arith
-  mk term.hasSymbols cvc5.Kind.NEG #[term.toUnsafe]
-
-
-/-- Builds a multiplication term.
-
-- Forbids difference logic.
-- Forces non-linear logic if non-linear.
--/
-def mkMul : Build (Term α) := do
-  let _ := h_size ; let _ := Arith
-  nonDiff
-  let hasSymbols ← checkNonLinearOfArgs terms
-  mk hasSymbols .MULT (terms.map toUnsafe)
-
-@[inherit_doc mkMul]
-def mul : Build (Term α) := mkMul #[lft, rgt]
-
-/-- Arithmetic division with division by `0` undefined, left associative.
-
-- Forbids difference logic.
-- Forces non-linear logic if non-linear.
--/
-def mkDiv! : Build (Term α) := do
-  let _ := h_size
-  nonDiff
-  let hasSymbols ← checkNonLinearOfArgs terms
-  let terms := terms.map toUnsafe
-  Arith.inspect
-    (fInt := fun _ => mk hasSymbols .INTS_DIVISION terms)
-    (fRat := fun _ => mk hasSymbols .DIVISION terms)
-
-@[inherit_doc mkDiv!]
-def div! : Build (Term α) := do
-  mkDiv! #[lft, rgt]
-
-/-- Arithmetic division with division by `0` defined to be `0`, left associative. -/
-def mkDivTotal : Build (Term α) := do
-  nonDiff
-  let hasSymbols ← checkNonLinearOfArgs #[lft, rgt]
-  let args := #[lft.toUnsafe, rgt.toUnsafe]
-  Arith.inspect
-    (fInt := fun _ => mk hasSymbols .INTS_DIVISION_TOTAL args)
-    (fRat := fun _ => mk hasSymbols .DIVISION_TOTAL args)
-
-@[inherit_doc mkDivTotal]
-def divTotal : Build (Term α) := mkDivTotal lft rgt
-
-end arith
-
-
-
-/-! ### Function application -/
-section apply
-
-/-- Flattens higher-order applications. -/
-private partial def flattenHoApply
-  (revArgs : Array cvc5.Term) (functionTerm : cvc5.Term)
-: Term.Build cvc5.Term := do
-  match functionTerm.getKind with
-  -- if `functionTerm` is a higher-order apply, deconstruct it
-  | .HO_APPLY =>
-    let args := functionTerm.getChildren
-    if h : 0 < args.size then
-      let functionTerm := args[0]
-      let args := args.toSubarray (start := 1)
-      let revArgs := revArgs |> args.foldr fun arg acc => acc.push arg
-      flattenHoApply revArgs functionTerm
-    else Cvc.throwInternal s!"cannot deconstruct `HO_APPLY` with no arguments"
-  -- otherwise reconstruct a normal application
-  | _ =>
-    if revArgs.isEmpty
-    then Cvc.throwInternal s!"unreachable: `flattenHoApply` with empty list of arguments"
-    else
-      let revArgs := revArgs.push functionTerm
-      -- build the unsafe term
-      managerDoM fun tm => tm.mkTerm cvc5.Kind.APPLY_UF revArgs.reverse
-
-/-- Applies a function term to an argument.
-
-## Partial applications and higher-order
-
-This function supports partial applications: they are encoded as `cvc5.Kind.HO_APPLY` terms, which
-**would** trigger errors if used in a solver without support for higher-order. Since support for
-higher-order makes cvc5-level reasoning much more expensive, we want to avoid having `HO_APPLY`
-terms as much as possible.
-
-For this reason, this function detects when it is building an application that yields a non-function
-term; in this case, it will destruct the underlying higher-order terms (recursively, and if any) and
-rewrite them as a regular (first-order) function application.
--/
-protected def apply [IsSrt β]
-  (function : Term (α → β)) (arg : Term α)
-: Term.Build (Term β) := do
-  let hasSymbols := function.hasSymbols ∨ arg.hasSymbols
-  let term! := function.toUnsafe
-  let sort! := term!.getSort
-  let dom ← sort!.getFunctionDomainSorts
-  if 1 < dom.size
-  then Term.mk hasSymbols .HO_APPLY #[function.toUnsafe, arg.toUnsafe]
-  else ofUnsafe hasSymbols <$> flattenHoApply #[arg.toUnsafe] term!
-
-end apply
+
+def Stx.ident := ``Term |> Lean.mkIdent
+
+/-- Constructor from an unsafe `cvc5` term. -/
+private def ofUnsafe (term : cvc5.Term) : Term := term
+
+section variable (term : Term)
+
+/-- Unsafe `cvc5` version of a `Term`. -/
+private def toUnsafe : cvc5.Term := term
+
+/-- The `Srt` of a term. -/
+abbrev srt : Env Srt := return term.toUnsafe.getSort |> Srt.ofUnsafe
+
+/-- SMT-LIB string representation. -/
+def toSmtString (term : Term) : Env String :=
+  return term.toUnsafe.toString
+
+end
+
+
+
+/-! ### Thread-unsafe functions and instances -/
+namespace ThreadUnsafe
+
+@[inherit_doc cvc5.Term.beq]
+def beq! (t t' : Term) : Bool := t.toUnsafe.beq t'
+
+/-- Hash of a term. -/
+-- @[inherit_doc cvc5.Term.hash]
+def hash! (t : Term) : UInt64 := t.toUnsafe.hash
+
+scoped instance : Hashable Term := inferInstanceAs <| Hashable cvc5.Term
+scoped instance : BEq Term := inferInstanceAs <| BEq cvc5.Term
+
+end ThreadUnsafe
+
+
+
+/-! ### Safe versions of thread-unsafe functions -/
+
+@[inherit_doc cvc5.Term.beq]
+def beq (t t' : Term) : Env Bool := return Term.ThreadUnsafe.beq! t t'
+
+/-- The hash of a term. -/
+-- @[inherit_doc cvc5.Term.hash]
+def hash (t : Term) : Env UInt64 := return Term.ThreadUnsafe.hash! t
+
+
+
+/-! ### Hash maps and sets -/
+
+open scoped ThreadUnsafe in
+/-- Hashmap for `Term`s. -/
+def HMap (α : Type) : Type := Std.HashMap Term α
+
+namespace HMap open scoped ThreadUnsafe variable (map : HMap α) open Std (HashMap)
+
+/-- Explicitly accesses the underlying hashmap. -/
+private def get : HMap α → HashMap Term α := id
+@[inherit_doc HashMap.emptyWithCapacity]
+def empty (capacity : Nat := 8) : HMap α := HashMap.emptyWithCapacity capacity
+@[inherit_doc HashMap.insert]
+def insert (key : Term) (val : α) : Env (HMap α) := return map.get.insert key val
+@[inherit_doc HashMap.erase]
+def erase (key : Term) : Env (HMap α) := return map.get.erase key
+@[inherit_doc HashMap.get?]
+def get? (key : Term) : Env (Option α) := return map.get.get? key
+@[inherit_doc HashMap.contains]
+def contains (key : Term) : Env Bool := return map.get.contains key
+@[inherit_doc HashMap.size]
+def size : Nat := map.get.size
+@[inherit_doc HashMap.isEmpty]
+def isEmpty : Bool := map.get.isEmpty
+@[inherit_doc HashMap.keys]
+def keys : List Term := map.get.keys
+@[inherit_doc HashMap.toList]
+def toList : List (Term × α) := map.get.toList
+
+@[inherit_doc HashMap.foldM]
+def foldM := @map.get.foldM
+@[inherit_doc HashMap.fold]
+def fold := @map.get.fold
+@[inherit_doc HashMap.forM]
+def forM := @map.get.forM
+@[inherit_doc HashMap.forIn]
+def forIn := @map.get.forIn
+
+instance : ForM m (HMap α) (Term × α) := HashMap.instForMProd
+instance : ForIn m (HMap α) (Term × α) := HashMap.instForInProd
+
+end HMap
+
+attribute [irreducible] HMap
+
+
+/-! ### Term constructors. -/
+
+
+
+/-! #### Lean-value injection -/
+
+@[inherit_doc Tm.mkBoolean]
+def bool (b : Bool) : Env Term :=
+  tmDoM fun tm => Term.ofUnsafe <$> tm.mkBoolean b
+
+@[inherit_doc Tm.mkInteger]
+def int (i : Int) : Env Term :=
+  tmDoM fun tm => Term.ofUnsafe <$> tm.mkInteger i
+
+@[inherit_doc Tm.mkReal]
+def rat (r : Rat) : Env Term :=
+  tmDoM fun tm => Term.ofUnsafe <$> tm.mkRealOfRat r
+
+@[inherit_doc Tm.mkReal]
+def real (num : Int) (den : Nat) (h : den ≠ 0 := by (try simp) <;> grind) : Env Term :=
+  tmDoM fun tm => Term.ofUnsafe <$> tm.mkReal num den
+
+
+
+/-! #### Constant symbol creation -/
+
+/-- Creates a constant symbol of some sort. -/
+def symbol (name : String) (sort : Srt) : Env Term :=
+  tmDoM fun tm => tm.mkConst sort name
+
+/-- Creates a constant Boolean symbol. -/
+def boolSymbol (name : String) : Env Term :=
+  Srt.bool >>= symbol name
+
+/-- Creates a constant integer symbol. -/
+def intSymbol (name : String) : Env Term :=
+  Srt.int >>= symbol name
+
+/-- Creates a constant real symbol. -/
+def realSymbol (name : String) : Env Term :=
+  Srt.real >>= symbol name
+
+/-- Creates a constant regular expression symbol. -/
+def regexSymbol (name : String) : Env Term :=
+  Srt.regex >>= symbol name
+
+/-- Creates a constant regular expression symbol. -/
+def roundingModeSymbol (name : String) : Env Term :=
+  Srt.roundingMode >>= symbol name
+
+/-- Creates a constant string symbol. -/
+def stringSymbol (name : String) : Env Term :=
+  Srt.string >>= symbol name
+
+
+
+/-! #### Composite term creation -/
+
+
+
+section variable (t t' : Term) (terms : Terms) (valid : 2 ≤ terms.size := by (try simp) <;> omega)
+
+@[inherit_doc Tm.mkTerm, specialize opIndices]
+def mk (op : Kind) (terms : Terms) (opIndices : Array Nat := #[]) : Env Term :=
+  if opIndices.isEmpty
+  then tmDoM fun tm => Term.ofUnsafe <$> tm.mkTerm op terms
+  else tmDoM fun tm => do
+    let op ← tm.mkOpOfIndices op opIndices
+    Term.ofUnsafe <$> tm.mkTermOfOp op terms
+
+def Stx.ident_mk := ``mk |> Lean.mkIdent
+
+section open Lean.Parser
+
+declare_syntax_cat op2Defs1
+
+scoped syntax (name := op2Defs1Stx)
+  term
+  ppLine ppIndent(docComment ppLine ident)
+  ppLine ppIndent(docComment ppLine ident)
+: op2Defs1
+
+scoped syntax (name := op2DefsStx)
+  "op2Defs" (ppLine ppIndent(op2Defs1))+
+: command
+
+@[command_elab op2DefsStx]
+def op2DefsElab : Lean.Elab.Command.CommandElab
+| `(op2Defs $[ $inners:op2Defs1 ]*
+) => do
+  let arrayId := ``Array |> Lean.mkIdent
+  let mut stxArray := Array.mkEmpty inners.size
+  for inner in inners do
+    let `(op2Defs1|
+      $op:term $nAryDoc:docComment $nAryId:ident $binaryDoc:docComment $binaryId:ident
+    ) := inner
+      | Lean.Elab.throwUnsupportedSyntax
+    let stx ← `(
+      $nAryDoc:docComment
+      def $nAryId [$(Scope.Stx.ident)] (terms : $arrayId $(Term.Stx.ident)) :
+        (valid : 2 ≤ terms.size := by (try simp) <;> omega) → $(Env.Stx.ident) $(Term.Stx.ident)
+      := fun _ => $(Term.Stx.ident_mk) $op terms
+
+      $binaryDoc:docComment
+      def $binaryId [$(Scope.Stx.ident)] (lft rgt : $(Term.Stx.ident)) :
+        $(Env.Stx.ident) $(Term.Stx.ident)
+      := $nAryId:ident #[lft, rgt]
+    )
+    stxArray := stxArray.push stx
+  for stx in stxArray do
+    Lean.Elab.Command.elabCommand stx
+| _ => Lean.Elab.throwUnsupportedSyntax
+
+end
+
+op2Defs
+  .EQUAL /-- N-ary equality. -/ mkEq /-- Binary equality. -/ eq
+  .DISTINCT /-- N-ary pairwise non-equality. -/ mkDistinct /-- Binary non-equality. -/ distinct
+  .IMPLIES /-- N-ary implication. -/ mkImplies /-- Binary implication. -/ implies
+  .AND /-- N-ary conjunction. -/ mkAnd /-- Binary conjunction. -/ and
+  .OR /-- N-ary disjunction. -/ mkOr /-- Binary disjunction. -/ or
+  .XOR /-- N-ary exclusive-or. -/ mkXor /-- Binary exclusive-or. -/ xor
+  .LT /-- N-ary less-than. -/ mkLt /-- Binary less-than. -/ lt
+  .LEQ /-- N-ary less-than-or-equal-to. -/ mkLe /-- Binary less-than-or-equal-to. -/ le
+  .GEQ /-- N-ary greater-than-or-equal-to. -/ mkGe /-- Binary greater-than-or-equal-to. -/ ge
+  .GT /-- N-ary greater-than. -/ mkGt /-- Binary greater-than. -/ gt
+  .ADD /-- N-ary addition. -/ mkAdd /-- Binary addition. -/ add
+  .MULT /-- N-ary multiplication. -/ mkMul /-- Binary multiplication. -/ mul
+  .DIVISION_TOTAL
+    /-- N-ary total **real** division, division by `0` is `0`, left-associative. -/
+    mkRealDivTotal
+    /-- Binary total **real** division, division by `0` is `0`. -/
+    realDivTotal
+  .DIVISION
+    /-- N-ary **real** division, division by `0` undefined, left-associative. -/
+    mkRealDiv
+    /-- Binary **real** division, division by `0` undefined. -/
+    realDiv
+  .INTS_DIVISION_TOTAL
+    /-- N-ary total **integer** division, division by `0` is `0`, left-associative. -/
+    mkIntDivTotal
+    /-- Binary total **integer** division, division by `0` is `0`. -/
+    intDivTotal
+  .INTS_DIVISION
+    /-- N-ary **integer** division, division by `0` undefined, left-associative. -/
+    mkIntDiv
+    /-- Binary **integer** division, division by `0` undefined. -/
+    intDiv
+  .SUB /-- N-ary division. -/ mkSub /-- Binary division. -/ sub
+
+/-- Boolean negation of a term. -/
+def not := mk .NOT #[t]
+
+/-- If-then-else. -/
+def ite (c t e : Term) := mk .ITE #[c, t, e]
+
+/-- Function application. -/
+def apply (f arg : Term) := mk .APPLY_UF #[f, arg]
+
+/-- Total division. -/
+def divTotal := mk .DIVISION_TOTAL #[t, t']
+
+/-- Unary minus. -/
+def neg := mk .NEG #[t]
+
+/-- Power of two of an integer term. -/
+def pow2 := mk .POW2 #[t]
+
+/-- Integer modulus, modulus by `0` undefined. -/
+def mod := mk .INTS_MODULUS #[t, t']
+
+/-- Integer modulus, modulus by `0` is zero. -/
+def modTotal := mk .INTS_MODULUS_TOTAL #[t, t']
+
+/-- Absolute value over integers/reals. -/
+def abs := mk .ABS #[t]
+
+/-- Arithmetic power over integers/reals, both terms must have the same sort. -/
+def pow := mk .POW #[t, t']
+
+/-- Exponential of a real term. -/
+def exp := mk .EXPONENTIAL #[t]
+
+/-- Sine of a real term. -/
+def sine := mk .SINE #[t]
+
+/-- Cosine of a real term. -/
+def cosine := mk .COSINE #[t]
+
+/-- Tangent of a real term. -/
+def tangent := mk .TANGENT #[t]
+
+/-- Secant of a real term. -/
+def secant := mk .SECANT #[t]
+
+/-- Cosecant of a real term. -/
+def cosecant := mk .COSECANT #[t]
+
+/-- Cotangent of a real term. -/
+def cotangent := mk .COTANGENT #[t]
+
+/-- Arc-sine of a real term. -/
+def arcSine := mk .ARCSINE #[t]
+
+/-- Arc-cosine of a real term. -/
+def arcCosine := mk .ARCCOSINE #[t]
+
+/-- Arc-tangent of a real term. -/
+def arcTangent := mk .ARCTANGENT #[t]
+
+/-- Arc-secant of a real term. -/
+def arcSecant := mk .ARCSECANT #[t]
+
+/-- Arc-cosecant of a real term. -/
+def arcCosecant := mk .ARCCOSECANT #[t]
+
+/-- Arc-cotangent of a real term. -/
+def arcCotangent := mk .ARCCOTANGENT #[t]
+
+/-- Square root of a real term. -/
+def sqrt := mk .SQRT #[t]
+
+/-- Divisibility-by-`k` predicate over integer terms. -/
+def divisible (k : Nat) := mk .DIVISIBLE #[t] (opIndices := #[k])
+
+
+
+/-! #### Lean-value extraction -/
+
+
+
+@[inherit_doc cvc5.Term.getBooleanValue?]
+def boolVal? (t : Term) : Env (Option Bool) :=
+  return t.toUnsafe.getBooleanValue?
+@[inherit_doc cvc5.Term.getBooleanValue?]
+def boolVal (t : Term) : Env Bool := do
+  if let some b ← t.boolVal? then return b
+  else throwUser "cannot retrieve `Bool` value of a non-constant term"
+
+@[inherit_doc cvc5.Term.getIntegerValue?]
+def intVal? (t : Term) : Env (Option Int) :=
+  return t.toUnsafe.getIntegerValue?
+@[inherit_doc cvc5.Term.getIntegerValue?]
+def intVal (t : Term) : Env Int := do
+  if let some b ← t.intVal? then return b
+  else throwUser "cannot retrieve `Int` value of a non-constant term"
+
+@[inherit_doc cvc5.Term.getRationalValue?]
+def ratVal? (t : Term) : Env (Option Rat) :=
+  return t.toUnsafe.getRationalValue?
+@[inherit_doc cvc5.Term.getRationalValue?]
+def ratVal (t : Term) : Env Rat := do
+  if let some b ← t.intVal? then return b
+  else throwUser "cannot retrieve `Rat` value of a non-constant term"
+
+end
 
 end Term
 
 
 
-/-- A term-value, as produced by `getValue`-like (SMT) function. -/
-structure Value (α : Type) where
-/-- Private constructor so that users can't compromise this type's semantics. -/
-private ofTerm ::
-  /-- Underlying term. -/
-  toTerm : Term α
+/-! ## Conversion to terms -/
 
-namespace Value
 
-protected def toString (value : Value α) : String := toString value.toTerm
 
-instance : ToString (Value α) := ⟨Value.toString⟩
+/-- Conversion class from `α` to `Term`, with a `σ`-context. -/
+class ToTermIn (σ α : Type) : Type where
+  /-- Conversion to a `Term` in a `Cvc.Scope`, with a `σ`-context. -/
+  toTermIn : [Cvc.Scope] → α → StateT σ Env Term
 
-/-- Boolean values. -/
-protected abbrev Bool := Value Bool
-/-- Integer values. -/
-protected abbrev Int := Value Int
-/-- Real/`Rat` values. -/
-protected abbrev Real := Value Rat
-/-- String values. -/
-protected abbrev String := Value String
-/-- Array values. -/
-protected abbrev Array (α β : Type) := Value (Cvc.TMap α β)
-/-- Sequence values. -/
-protected abbrev Seq (α : Type) := Value (Array α)
-/-- Function values. -/
-protected abbrev Fun (α β : Type) := Value (α → β)
-/-- Product values. -/
-protected abbrev Prod (α β : Type) := Value (α × β)
+@[inherit_doc ToTermIn.toTermIn]
+def toTermIn := @ToTermIn.toTermIn
 
-section variable [A : IsSrt α] (value : Value α)
+/-- Context-free conversion class from `α` to `Term`.
 
-abbrev srt : (value : Value α) → Srt := 𝕂 A.srt
-
-theorem srt_bij : α = value.srt := A.h_bij
-
-def retype : Value value.srt := value.srt_bij ▸ value
-
-def inspectSrt (f : (srt : Srt) → Value srt → β) : β :=
-  f value.srt value.retype
-
-end
-
-def boolVal (value : Value.Bool) : Res Bool := value.toTerm.boolVal
-def intVal (value : Value.Int) : Res Int := value.toTerm.intVal
-def ratVal (value : Value.Real) : Res Rat := value.toTerm.ratVal
-
-end Value
-
-
-
-namespace Conv
-
-class ValueToVal (m : Type → Type) (α : Type) extends IsSrt α where
-mk' ::
-  Val : Type
-  ofValue : Value α → m Val
-
-namespace ValueToVal
-
-protected abbrev Id (α : Type) [IsSrt α] : ValueToVal Id α := ⟨Value α, id⟩
-
-def mk [IsSrt α] (Val : Type) (ofValue : Value α → m Val) : ValueToVal m α :=
-  ⟨Val, ofValue⟩
-
-def mkId [IsSrt α] : ValueToVal Id α := ⟨Value α, id⟩
-
-instance : CoeSort (ValueToVal m α) Type := ⟨fun conv => conv.Val⟩
-
-abbrev adaptM [A : ValueToVal m α]
-  (lift : {β : Type} → m β → m' β)
-: ValueToVal m' α := ⟨A.Val, lift ∘ A.ofValue⟩
-
-protected abbrev liftM [MonadLiftT m m'] [A : ValueToVal m α] : ValueToVal m' α :=
-  A.adaptM liftM
-
-instance defaultInstUnit : ValueToVal Id Unit := mk Unit fun _ => pure ()
-instance defaultInstBool : ValueToVal Res Bool := mk Bool fun v => v.boolVal
-instance : ToString defaultInstBool.Val := inferInstanceAs (ToString Bool)
-instance defaultInstInt : ValueToVal Res Int := mk Int fun v => v.intVal
-instance : ToString defaultInstInt.Val := inferInstanceAs (ToString Int)
-instance defaultInstRat : ValueToVal Res Rat := mk Rat fun t => t.ratVal
-instance : ToString defaultInstRat.Val := inferInstanceAs (ToString Rat)
-instance defaultInstString : ValueToVal Id String := mkId
-instance defaultInstRoundingMode : ValueToVal Id RoundingMode := mkId
-instance defaultInstRegex : ValueToVal Id Cvc.Regex := mkId
-
-instance defaultInstFloat : ValueToVal Id (Cvc.AnyFloat exp sig) := mkId
-instance defaultInstAbstract : ValueToVal Id (Cvc.Abstract k) := mkId
-instance defaultInstFiniteField : ValueToVal Id (Cvc.FiniteField n) := mkId
-instance defaultInstBitVec : ValueToVal Id (BitVec size) := mkId
-instance defaultInstUninterpreted : ValueToVal Id (Uninterpreted name) := mkId
-
-section variable [IsSrt α] [IsSrt β]
-
-instance defaultInstArray : ValueToVal Id (Array α) := mkId
-instance defaultInstProd : ValueToVal Id (α × β) := mkId
-instance defaultInstFun : ValueToVal Id (α → β) := mkId
-instance defaultInstTMap : ValueToVal Id (Cvc.TMap α β) := mkId
-instance defaultInstBag : ValueToVal Id (Cvc.Bag α) := mkId
-instance defaultInstSet : ValueToVal Id (Cvc.Set α) := mkId
-
-end
-
-abbrev defaultFor : (srt : Srt) → ValueToVal Res srt
-| .abstract _kind => defaultInstAbstract.adaptM .ok
-| .array _idx _elm =>
-  -- let (_, _) := (defaultFor idx, defaultFor elm)
-  defaultInstTMap.adaptM .ok
-| .bag _elm =>
-  -- let _ := defaultFor elm
-  defaultInstBag.adaptM .ok
-| .bool => defaultInstBool
-| .bitVec _n => defaultInstBitVec.adaptM .ok
-| .finiteField _n => defaultInstFiniteField.adaptM .ok
-| .float _exp _sig => defaultInstFloat.adaptM .ok
-| .function _dom _cod =>
-  -- let (_, _) := (defaultFor dom, defaultFor cod)
-  defaultInstFun.adaptM .ok
-| .int => defaultInstInt
-| .prod _lft _rgt =>
-  -- let (_, _) := (defaultFor lft, defaultFor rgt)
-  defaultInstProd.adaptM .ok
-| .real => defaultInstRat
-| .regex => defaultInstRegex.adaptM .ok
-| .roundingMode => defaultInstRoundingMode.adaptM .ok
-| .seq _elm =>
-  -- let _ := defaultFor elm
-  defaultInstArray.adaptM .ok
-| .set _elm =>
-  -- let _ := defaultFor elm
-  defaultInstSet.adaptM .ok
-| .string => defaultInstString.adaptM .ok
-| .unit => defaultInstUnit.adaptM .ok
-| .uninterpreted _ => defaultInstUninterpreted.adaptM .ok
-
-namespace Default
-
-scoped instance (srt : Srt) : ValueToVal Res srt := defaultFor srt
-
-end Default
-
-end ValueToVal
-
-
-
-class ValuesToVal (m : Type → Type) where
-  instValueToVal : (srt : Srt) → ValueToVal m srt
-
-namespace ValuesToVal
-
-protected abbrev Values : ValuesToVal Id := ⟨(ValueToVal.Id ·)⟩
-
-protected abbrev Default : ValuesToVal Res where
-  instValueToVal := ValueToVal.defaultFor
-
-end ValuesToVal
-
-end Conv
-
-
-
-/-! ## Conversion of *term-values* -/
-
-class Srt.ToValType where
-  Val : Srt → Type
-
-def Srt.ToValType.Terms : ToValType where
-  Val (srt : Srt) := Term srt
-
-namespace Term
-
-class ToVals extends toValConv : Srt.ToValType where
-  build : (srt : Srt) → Term srt → Val srt
-
-def ToVals.Terms : ToVals where
-  toValConv := .Terms
-  build := fun _ => id
-
--- def ToVals.Default : ToVals where
-
-namespace ToVals
-
--- protected def Terms :
-
-end ToVals
-
-end Term
-
-
-
-/-! ## `Smt` environment and functions -/
-
-structure Smt.State where
-  solver : cvc5.Solver
-  builder : Term.Build.State
-  private nextActlitIdx' : Nat
-
-abbrev SmtT (m : Type → Type) :=
-  ResT (StateT Smt.State m)
-
-abbrev SmtIO := SmtT IO
-
-abbrev Smt := SmtT Id
-
-namespace Smt variable [Monad m]
-
-instance : MonadLift ResIO SmtIO where
-  monadLift code state := return (← code, state)
-
-instance : MonadLift m (SmtT m) := ⟨fun code state => return (.ok (← code), state)⟩
-
-instance [Monad m] [Monad m'] [MonadLift m m'] : MonadLift (SmtT m) (SmtT m') :=
-  ⟨fun code state => return ← code state⟩
-
-instance [Monad m] : MonadLift Smt (SmtT m) :=
-  ⟨fun code state => return code state⟩
-
-instance [Monad m] [MonadLiftT IO m] : MonadLift SmtIO (SmtT m) :=
-  ⟨fun code state => return ← code state⟩
-
-instance [Monad m] : MonadLift Term.Build (SmtT m) where
-  monadLift build := do
-    let res ← modifyGet fun state =>
-      let (res, builder) := build state.builder
-      (res, {state with builder})
-    res
-
-def nextActlitIdx : Smt Nat :=
-  modifyGetThe Smt.State fun state =>
-    let idx := state.nextActlitIdx'
-    (idx, {state with nextActlitIdx' := idx.succ})
-
-private def lift5 [Monad m] (code : cvc5.SolverT m α) : SmtT m α := do
-  let state ← getThe Smt.State
-  let (res, solver) ← code state.solver
-  set {state with solver}
-  return ← res
-
-/-- Sets an option in the solver. -/
-def setOption (opt : Cvc.Option) : Smt Unit := do
-  let (key, val) := opt.keyVal
-  let state ← getThe Smt.State
-  let (res, solver) ← cvc5.Solver.setOption key val state.solver
-  let () ← res
-  set {state with solver}
-
-
-/-- Declares a function symbol. -/
-def declare (symbol : String) (α : Type) [IsSrt α] : Smt (Term α) := do
-  let srt := getSrt α
-  let (doms, cod) ← srt.toSignature!
-  let f ← lift5 <| cvc5.Solver.declareFun symbol doms cod
-  return Term.ofUnsafe true f
-
-@[inherit_doc declare]
-def declare' {α : Type} [IsSrt α] (symbol : String) : Smt (Term α) :=
-  declare symbol α
-
-/-- Asserts a formula. -/
-def assert (formula : Formula) : Smt Unit := do
-  lift5 <| cvc5.Solver.assertFormula formula.toUnsafe
-
-section variable (assuming : Option (Array Formula) := none)
-
-/-- Checks the satisfiability of the formulas asserted with `Smt.assert`. -/
-def checkSat : Smt CheckSat := do
-  let res ←
-    match assuming with
-    | none | some #[] =>
-      cvc5.Solver.checkSat |> lift5
-    | some assuming =>
-      assuming.map Term.toUnsafe |> cvc5.Solver.checkSatAssuming |> lift5
-  pure <|
-    if res.isSat then CheckSat.sat
-    else if res.isUnsat then CheckSat.unsat
-    else if res.isUnknown then CheckSat.unknown res.toString
-    else CheckSat.other res.toString
-
-/-- Simplified `Smt.checkSat`, returns true/false for sat/unsat, `none` for unknown/unexpected. -/
-def checkSat? : Smt (Option Bool) :=
-  CheckSat.isSat? <$> checkSat assuming
-
-end
-
-
-
-
-/-- Sat-mode state. -/
-structure Sat.State extends Smt.State where
-/-- Constructor. -/
-private mk ::
-
-/-- Unsat-mode state. -/
-structure Unsat.State extends Smt.State where
-/-- Constructor. -/
-private mk ::
-
-/-- Unknown-mode state. -/
-structure Unknown.State extends Smt.State where
-/-- Constructor. -/
-private mk ::
-
-/-- Sat-mode monad, allows running commands such as get-value.
-
-`Smt` does not lift to this monad as this would allow issuing a check-sat that could switch to a
-different solver mode.
+See also `ToTermMin`.
 -/
-abbrev SatT (m : Type → Type u) :=
-  ResT (StateT Sat.State m)
+class ToTerm (α : Type) : Type where
+  /-- Context-free conversion to a `Term` in a `Cvc.Scope`. -/
+  toTerm : [Cvc.Scope] → α → Env Term
 
-@[inherit_doc SatT]
-abbrev Sat := SatT (m := Id)
+@[inherit_doc ToTerm.toTerm]
+def toTerm := @ToTerm.toTerm
 
-def Sat.unexpected : SatT m α :=
-  Error.throwUser "unexpected sat result"
+namespace ToTerm
 
-/-- Unsat-mode monad, allows running commands such as get-proof.
+instance toToTermIn [ToTerm α] : ToTermIn Unit α where
+  toTermIn | a, state => return (← toTerm a, state)
 
-`Smt` does not lift to this monad as this would allow issuing a check-sat that could switch to a
-different solver mode.
--/
-abbrev UnsatT (m : Type → Type u) :=
-  ResT (StateT Unsat.State m)
-
-@[inherit_doc UnsatT]
-abbrev Unsat := UnsatT (m := Id)
-
-def Unsat.unexpected : UnsatT m α :=
-  Error.throwUser "unexpected unsat result"
-
-/-- Unknown-mode monad, allows running unknown-mode-specific commands.
-
-`Smt` does not lift to this monad as this would allow issuing a check-sat that could switch to a
-different solver mode.
--/
-abbrev UnknownT (m : Type → Type u) :=
-  ResT (StateT Unknown.State m)
-
-@[inherit_doc UnknownT]
-abbrev Unknown := UnknownT (m := Id)
-
-def Unknown.unexpected : UnknownT m α :=
-  Error.throwUser "unexpected unknown result"
+end ToTerm
 
 
 
-/-- Performs a check-sat and runs sat/unsat/unknown-specific code. -/
-def checkSatAnd
-  (assuming : Option (Array Formula) := none)
-  (ifSat : Smt.SatT m α := Sat.unexpected)
-  (ifUnsat : Smt.UnsatT m α := Unsat.unexpected)
-  (ifUnknown : Smt.UnknownT m α := Unknown.unexpected)
-: SmtT m α := do
-  if let some isSat ← checkSat? assuming then
-    let state ← getThe Smt.State
-    if isSat then
-      let (res, state) ← ifSat ⟨state⟩
-      set state.toState
-      return ← res
-    else
-      let (res, state) ← ifUnsat ⟨state⟩
-      set state.toState
-      return ← res
-  else
-    let state ← getThe Smt.State
-    let (res, state) ← ifUnknown ⟨state⟩
-    set state.toState
-    return ← res
+/-! ## Proof and proof rules -/
+
+@[inherit_doc cvc5.Proof]
+def Proof [Cvc.Scope] : Type := cvc5.Proof
+
+namespace Proof variable [Cvc.Scope] (proof : Proof)
+
+@[inherit_doc cvc5.ProofRule]
+abbrev Rule := cvc5.ProofRule
+
+@[inherit_doc cvc5.ProofRewriteRule]
+abbrev RwRule := cvc5.ProofRewriteRule
+
+/-- Constructor from an unsafe `cvc5` proof. -/
+private def ofUnsafe (proof : cvc5.Proof) : Proof := proof
+
+/-- Unsafe `cvc5` version of a `Proof`. -/
+def toUnsafe : cvc5.Proof := proof
+
+@[inherit_doc cvc5.Proof.getRule]
+def getRule : Env Rule := return proof.toUnsafe.getRule
+
+@[inherit_doc cvc5.Proof.getRewriteRule]
+def getRewriteRule : Env RwRule := proof.toUnsafe.getRewriteRule
+
+@[inherit_doc cvc5.Proof.getResult]
+def getResult : Env Term := return proof.toUnsafe.getResult
+
+@[inherit_doc cvc5.Proof.getChildren]
+def getChildren : Env (Array Proof) := return proof.toUnsafe.getChildren
+
+@[inherit_doc cvc5.Proof.getArguments]
+def getArguments : Env Terms := return proof.toUnsafe.getArguments
+
+end Proof
+
+
+
+/-- A cvc5 solver instance. -/
+structure Solver [Cvc.Scope] : Type where
+private mk' ::
+  get : cvc5.Solver
+  log? : IO.Ref Bool
+  logRef : IO.Ref String
+
+
+
+namespace Env variable [Cvc.Scope]
+
+def SatT (m : Type → Type) (α : Type) := EnvT m α
+abbrev Sat (α : Type) := SatT BaseIO α
+
+def UnsatT (m : Type → Type) (α : Type) := EnvT m α
+abbrev Unsat (α : Type) := UnsatT BaseIO α
+
+def UnknownT (m : Type → Type) (α : Type) := EnvT m α
+abbrev Unknown (α : Type) := UnknownT BaseIO α
+
+section variable [Monad m]
 
 namespace Sat
+instance : Monad (SatT m) := inferInstanceAs <| Monad <| EnvT m
+instance : MonadExcept Error (SatT m) := inferInstanceAs <| MonadExcept Error <| EnvT m
+instance : MonadLift (EnvT m) (SatT m) := ⟨id⟩
+example [MonadLiftT BaseIO m] : MonadLiftT Sat (SatT m) := ⟨fun code state => code state⟩
+--sanity
+example : MonadLiftT m (SatT m) := inferInstance
+example : MonadLiftT Env Sat := inferInstance
 
-instance [Monad m] : MonadLift Smt.Sat (Smt.SatT m) :=
-  ⟨fun code state => return code state⟩
-instance [Monad m] : MonadLift Term.Build (Smt.SatT m) := ⟨fun build => do
-  let res ← modifyGet fun state =>
-    let (res, builder) := build state.builder
-    (res, {state with builder})
-  res
-⟩
-
-/-- Unsafe solver monad lift. -/
-private def lift5 (code : cvc5.SolverT m α) : SatT m α := fun state => do
-  let (res, solver) ← code state.solver
-  return (Res.lift res, {state with solver})
-
-/-- Retrieves the value of a term in `Sat` mode.
-
-This function is available the following namespaces: `Cvc.Term`, `Cvc.Smt`, and `Cvc.Smt.Sat`.
--/
-def getValue (term : Term α) : Sat (Value α) := do
-  let term! ← lift5 <| cvc5.Solver.getValue (m := Id) term.toUnsafe
-  return Term.ofUnsafe false term! |> Value.ofTerm
-
-/-- Retrieves the values of some terms of the same sort in `Sat` mode.
-
-This function is available the following namespaces: `Cvc.Term`, `Cvc.Smt`, and `Cvc.Smt.Sat`.
--/
-def getValues (terms : Array (Term α)) : Sat (Array (Term α × Value α)) := do
-  let mut values := Array.mkEmpty terms.size
-  for term in terms do
-    let value ← getValue term
-    values := values.push (term, value)
-  return values
-
-/-- Retrieves the *concrete `Val`ue* of a term in `Sat` mode. -/
-def getValUsing [Monad m] [MonadLiftT m Sat]
-  (Val : Conv.ValueToVal m α) (term : Term α)
-: Sat Val :=
-  getValue term >>= liftM ∘ Val.ofValue
-
-@[inherit_doc getValUsing]
-def getVal [Monad m] [MonadLiftT m Sat] [Val : Conv.ValueToVal m α] (term : Term α) : Sat Val :=
-  getValUsing Val term
-
-/-- Retrieves the *concrete values* of some terms of the same sort in `Sat` mode. -/
-def getValsUsing (Val : Conv.ValueToVal Sat α) (terms : Array (Term α))
-: Sat (Array (Term α × Val)) := do
-  let mut values := Array.mkEmpty terms.size
-  for term in terms do
-    let value ← getVal term
-    values := values.push (term, value)
-  return values
-
-@[inherit_doc getValsUsing]
-def getVals [Val : Conv.ValueToVal Sat α] (terms : Array (Term α)) : Sat (Array (Term α × Val)) :=
-  getValsUsing Val terms
-
+/-- Reports an unexpected result. -/
+def unexpected : SatT m α := throwUser "unexpected *sat* result"
 end Sat
 
-export Sat (getValue getValues getValUsing getValsUsing getVal getVals)
-
-
-
 namespace Unsat
+instance : Monad (UnsatT m) := inferInstanceAs <| Monad <| EnvT m
+instance : MonadExcept Error (UnsatT m) := inferInstanceAs <| MonadExcept Error <| EnvT m
+instance : MonadLift (EnvT m) (UnsatT m) := ⟨id⟩
+example [MonadLiftT BaseIO m] : MonadLiftT Unsat (UnsatT m) := ⟨fun code state => code state⟩
+--sanity
+example : MonadLiftT m (UnsatT m) := inferInstance
+example : MonadLiftT Env Unsat := inferInstance
 
-instance [Monad m] : MonadLift Smt.Unsat (Smt.UnsatT m) :=
-  ⟨fun code state => return code state⟩
-instance [Monad m] : MonadLift Term.Build (Smt.UnsatT m) := ⟨fun build => do
-  let res ← modifyGet fun state =>
-    let (res, builder) := build state.builder
-    (res, {state with builder})
-  res
-⟩
-
-/-- Unsafe solver monad lift. -/
-private def lift5 (code : cvc5.SolverT m α) : UnsatT m α := fun state => do
-  let (res, solver) ← code state.solver
-  return (Res.lift res, {state with solver})
-
-/-- Retrieves the unsat-proofs in `Unsat` mode. -/
-def getProof : Unsat (Array cvc5.Proof) := do
-  lift5 <| cvc5.Solver.getProof
-
+/-- Reports an unexpected result. -/
+def unexpected : UnsatT m α := throwUser "unexpected *unsat* result"
 end Unsat
 
-export Unsat (getProof)
-
-
-
 namespace Unknown
+instance : Monad (UnknownT m) := inferInstanceAs <| Monad <| EnvT m
+instance : MonadExcept Error (UnknownT m) := inferInstanceAs <| MonadExcept Error <| EnvT m
+instance : MonadLift (EnvT m) (UnknownT m) := ⟨id⟩
+example [MonadLiftT BaseIO m] : MonadLiftT Unknown (UnknownT m) := ⟨fun code state => code state⟩
+--sanity
+example : MonadLiftT m (UnknownT m) := inferInstance
+example : MonadLiftT Env Unknown := inferInstance
 
-instance [Monad m] : MonadLift Smt.Unknown (Smt.UnknownT m) :=
-  ⟨fun code state => return code state⟩
-instance [Monad m] : MonadLift Term.Build (Smt.UnknownT m) := ⟨fun build => do
-  let res ← modifyGet fun state =>
-    let (res, builder) := build state.builder
-    (res, {state with builder})
-  res
-⟩
-
-/-- Unsafe solver monad lift. -/
-private def lift5 (code : cvc5.SolverT m α) : UnknownT m α := fun state => do
-  let (res, solver) ← code state.solver
-  return (Res.lift res, {state with solver})
-
+/-- Reports an unexpected result. -/
+def unexpected : UnknownT m α := throwUser "unexpected *unknown* result"
 end Unknown
 
-end Smt
+end
+
+end Env
 
 
 
-namespace Term
+namespace Solver variable [Cvc.Scope]
 
-export Smt (getValue getValues getVal getValUsing getVals getValsUsing)
-
-namespace ToVal
-export Term (getVal getValUsing getVals getValsUsing)
-end ToVal
-
-/-- Returns the symbol of a symbol-term. -/
-def getSymbol? (term : Term α) : Option String :=
-  term.toUnsafe.getSymbol?
-
-end Term
+/-- Constructor from a unsafe `cvc5` solver. -/
+private def ofUnsafe (name : String) (solver : cvc5.Solver) : Env Solver :=
+  return ⟨solver, ← IO.mkRef false, ← IO.mkRef s!"; log for `{name}`"⟩
 
 
+section variable (solver : Solver)
 
-namespace SmtT variable [M : Monad m]
+def getLog : Env String := solver.logRef.get
 
-def runWith' (smt : SmtT m α) (state : Smt.State) : m (Except Error α × Smt.State) :=
-  smt state
+def log (lazy : Unit → Env String) : Env Unit := do
+  if ← solver.log?.get then
+    solver.logRef.modifyGet ((), s!"{·}\n\n{← lazy ()}")
 
-def runWith (smt : SmtT m α) (state : Smt.State) : m (Except Error α) :=
-  Prod.fst <$> smt.runWith' state
+def logComment (lazy : Unit → String) : Env Unit := do
+  if ← solver.log?.get then
+    let lines := lazy () |>.splitOn "\n"
+    solver.logRef.modifyGet fun s => ((), lines.foldl (init := s ++ "\n") (s!"{·}\n; {·}"))
 
-def run' [MonadLiftT BaseIO m]
-  (smt : SmtT m α) (state? : Option Smt.State := none)
-: m (Except Error (α × Smt.State)) := do
-  if let some state := state? then
-    let (res, state) ← smt.runWith' state
-    return res.map (·, state)
-  else
-    let tm ← cvc5.TermManager.new
-    let builder := Term.Build.State.ofManager tm
-    let res ← cvc5.Solver.run builder.manager fun solver => do
-      let (res, state) ← smt ⟨solver, builder, 0⟩
-      return (.ok (res, state), solver)
-    match res with
-    | .ok (.ok res, state) => return .ok (res, state)
-    | .ok (.error err, _) => return .error err
-    | .error err => return .error <| Error.ofCvc5 err
+/-- Unsafe `cvc5` version of a `Solver`. -/
+private def toUnsafe : cvc5.Solver := solver.get
 
-abbrev run [MonadLiftT BaseIO m]
-  (smt : SmtT m α) (state? : Option Smt.State := none)
-: m (Except Error α) := do
-  Except.map Prod.fst <$> smt.run' state?
+def logCommands (on : Bool := true) : Env Unit :=
+  solver.log?.set on
 
-def runIO' (smt : SmtIO α) (state? : Option Smt.State := none) : IO (α × Smt.State) := do
-  match ← smt.run' state? with
-  | .ok res => return res
-  | .error err =>
-    IO.eprintln s!"{err}"
-    throw <| IO.Error.userError err.toString
 
-def runIO (smt : SmtIO α) (state? : Option Smt.State := none) : IO α :=
-  Prod.fst <$> smt.runIO' state?
 
-def runWithBuilder'
-  (smt : SmtT m α) (builder : Term.Build.State)
-: m (Except Error (α × Smt.State)) := do
-  let res ← cvc5.Solver.run builder.manager fun solver => do
-    let (res, state) ← smt.runWith' ⟨solver, builder, 0⟩
-    return (.ok (res.map (·, state)), state.solver)
-  match res with
-  | .ok (.ok (res, state)) => return .ok (res, state)
-  | .ok (.error err) => return .error err
-  | .error err => return .error <| Error.ofCvc5 err
+/-- Constructor. -/
+def mk (name : String := "cvc5") (log? : Bool := false) : Env Solver := do
+  let solver ← (tmDoM fun tm => cvc5.Solver.new tm) >>= ofUnsafe name
+  solver.logCommands log?
+  return solver
 
-def runWithBuilder (smt : SmtT m α) (builder : Term.Build.State) : m (Except Error α) :=
-  Except.map Prod.fst <$> smt.runWithBuilder' builder
+@[inherit_doc cvc5.Solver.parseCommands]
+def parseSmtLib (smtLib : String) : Env Unit :=
+  (fun _ => ()) <$> solver.toUnsafe.parseCommands smtLib
 
-end SmtT
+@[inherit_doc cvc5.Solver.setOption]
+def setOption (opt val : String) : Env Unit := do
+  let mut passAlong := true
+  if opt = "log" then
+    passAlong := false
+    match val with
+    | "true" => solver.logCommands true
+    | "false" => solver.logCommands false
+    | s => throwUser s!"expected `true` or `false` as value for option `log`, got `{s}`"
+  solver.log fun () => return s!"(set-option :{opt} {val})"
+  if passAlong then solver.toUnsafe.setOption opt val
 
-namespace Smt
-export SmtT (runWith' runWith run' run runIO' runIO runWithBuilder' runWithBuilder)
-end Smt
+@[inherit_doc cvc5.Solver.setLogic]
+def setLogic (logic : Logic) : Env Unit := do
+  solver.log fun () => return s!"(set-logic {logic.toSmtLib})"
+  solver.toUnsafe.setLogic logic.toSmtLib
+
+section variable (symbol : String)
+
+@[inherit_doc cvc5.Solver.declareFun]
+def declareFun (sorts : Array Srt) (sort : Srt) : Env Term :=
+  Term.ofUnsafe <$> solver.toUnsafe.declareFun symbol sorts sort
+
+/-- Declares a constant symbol. -/
+def declareConst (sort : Srt) : Env Term :=
+  solver.declareFun symbol #[] sort
+
+/-- Declares a Boolean symbol. -/
+def declareBool : Env Term := Srt.bool >>= solver.declareConst symbol
+/-- Declares an integer symbol. -/
+def declareInt : Env Term := Srt.int >>= solver.declareConst symbol
+/-- Declares a real symbol. -/
+def declareReal : Env Term := Srt.real >>= solver.declareConst symbol
+/-- Declares a string symbol. -/
+def declareString : Env Term := Srt.string >>= solver.declareConst symbol
+
+end
+
+@[inherit_doc cvc5.Solver.resetAssertions]
+def resetAssertions : Env Unit := do
+  solver.log fun () => return s!"(reset)"
+  solver.toUnsafe.resetAssertions
+
+@[inherit_doc cvc5.Solver.assertFormula]
+def assert (term : Term) : Env Unit := do
+  solver.log fun () => return s!"(assert {← term.toSmtString})"
+  solver.toUnsafe.assertFormula term
+
+/-- Asserts a term `t` under an activation term `act`: same as `assert`-ing `act → t`. -/
+def activeAssert (act : Term) (t : Term) : Env Unit :=
+  act.implies t >>= solver.assert
+
+@[inherit_doc cvc5.Solver.checkSatAssuming]
+def checkSat? (assuming : Terms := #[]) : Env CheckSat := do
+  let res ← .ofUnsafe <$> solver.toUnsafe.checkSatAssuming assuming
+  solver.log fun () => do
+    if assuming.isEmpty then return s!"(check-sat)\n; {res}"
+    else
+      let mut s := "(check-sat-assuming ("
+      for t in assuming do
+        s := s!"{s}\n  {← t.toSmtString}"
+      return s!"{s}\n))\n; {res}"
+  return res
+
+/-- Check-sat with optional assumptions and runs sat/unsat/unknown-mode-specific code. -/
+def checkSatM [Monad m] [MonadLiftT BaseIO m]
+  (assuming : Terms := #[])
+  (ifSat : Env.SatT m α := Env.Sat.unexpected)
+  (ifUnsat : Env.UnsatT m α := Env.Unsat.unexpected)
+  (ifUnknown : Env.UnknownT m α := Env.Unknown.unexpected)
+: EnvT m α := do
+  match ← solver.checkSat? assuming with
+  | .sat => ifSat
+  | .unsat => ifUnsat
+  | .unknown _ | .other _ => ifUnknown
+
+@[inherit_doc checkSatM]
+def checkSat
+  (assuming : Terms := #[])
+  (ifSat : Env.Sat α := Env.Sat.unexpected)
+  (ifUnsat : Env.Unsat α := Env.Unsat.unexpected)
+  (ifUnknown : Env.Unknown α := Env.Unknown.unexpected)
+: Env α :=
+  checkSatM (m := BaseIO) solver assuming ifSat ifUnsat ifUnknown
+
+/-! ### Sat-mode-specific commands -/
+section satMode
+
+@[inherit_doc cvc5.Solver.getValue]
+def getValue (term : Term) : Env.Sat Term := do
+  solver.log fun () => return s!"(get-value\n  {← term.toSmtString}\n)"
+  solver.toUnsafe.getValue term
+
+@[inherit_doc cvc5.Solver.getValues]
+def getValues (terms : Terms) : Env.Sat Terms := do
+  solver.log fun () => do
+    let mut s := "(get-values"
+    for t in terms do
+      s := s!"{s}\n  {← t.toSmtString}"
+    return s ++ "\n)"
+  solver.toUnsafe.getValues terms
+
+/-- Same as `getValues` but produces a map from terms to their value. -/
+def getValueMap (terms : Terms) : Env.Sat (Term.HMap Term) := do
+  Term.HMap.empty terms.size
+  |> terms.foldlM fun map term => solver.getValue term >>= map.insert term
+
+@[inherit_doc cvc5.Solver.getModelDomainElements]
+def getDomainElements (sort : Srt) : Env.Sat Terms := solver.toUnsafe.getModelDomainElements sort
+
+end satMode
+
+
+
+/-! ### Unsat-mode-specific commands -/
+section unsatMode
+
+@[inherit_doc cvc5.Solver.getUnsatCore]
+def getUnsatCore : Env.Unsat Terms := do
+  solver.log fun () => return s!"(get-unsat-core)"
+  solver.toUnsafe.getUnsatCore
+
+@[inherit_doc cvc5.Solver.getProof]
+def getProof : Env.Unsat (Array Proof) := do
+  solver.log fun () => return s!"(get-proof)"
+  solver.toUnsafe.getProof
+
+@[inherit_doc cvc5.Solver.proofToString]
+def proofToString (proof : Proof) : Env.Unsat String := solver.toUnsafe.proofToString proof
+
+end unsatMode
+
+/-- Performs a check-sat, if *unsat* runs get-unsat-core. -/
+def checkUnsatCore? (assuming : Terms := #[]) : Env (Option Terms) :=
+  solver.checkSat assuming (ifSat := return none) (ifUnsat := some <$> solver.getUnsatCore)
+
+end
+
+end Solver
+
+
+
+attribute [irreducible] Srt
+attribute [irreducible] Term
+attribute [irreducible] Proof
+
+-- attribute [irreducible] EnvT
+-- attribute [irreducible] Env.SatT
+-- attribute [irreducible] Env.UnsatT
+-- attribute [irreducible] Env.UnknownT
