Cvc/Basic/Basic.lean
@@ -1,0 +1,75 @@
+/-
+Copyright (c) 2025 by the authors listed in the file AUTHORS and their
+institutional affiliations. All rights reserved.
+Released under Apache 2.0 license as described in the file LICENSE.
+Authors: Adrien Champion
+-/
+
+import cvc5
+
+
+
+/-! # Basic helpers -/
+namespace Cvc
+
+export cvc5 (Kind SortKind)
+
+
+
+/-- The constant combinator. -/
+abbrev 𝕂 (val : α) (_ : β) : α := val
+
+
+
+/-- Lazy string interpolation: `fun () => s!<interp>`. -/
+macro:max "ls!" str:interpolatedStr(term) : term
+  => `( (fun () => s!$str : Unit → String)  )
+
+
+
+/-- A check-sat result.-/
+inductive CheckSat
+/-- Formulas asserted are satisfiable, *i.e.* a model exists. -/
+| sat
+/-- Formulas are unsatisfiable, no assignment of the symbols makes them true. -/
+| unsat
+/-- Solver returned unknown. -/
+| unknown (desc : String)
+/-- Solver returned some unexpected, non-error result. -/
+| other (desc : String)
+
+namespace CheckSat
+
+/-- Conversion to a simple *is sat?* flag, `none` on unknown/unexpected results. -/
+def isSat? : CheckSat → Option Bool
+| sat => true
+| unsat => false
+| unknown _ | other _ => none
+
+/-- True iff the result is sat. -/
+def isSat (res : CheckSat) : Bool := res.isSat?.getD false
+
+/-- Conversion to a simple *is unsat?* flag, `none` on unknown/unexpected results. -/
+def isUnsat? (cs : CheckSat) : Option Bool :=
+  Bool.not <$> cs.isSat?
+
+/-- True iff the result is sat. -/
+def isUnsat (res : CheckSat) : Bool := res.isUnsat?.getD false
+
+/-- Conversion from a `cvc5` result. -/
+def ofUnsafe (result : cvc5.Result) : CheckSat :=
+  if result.isSat then .sat
+  else if result.isUnsat then .unsat
+  else if let some unkTxt := result.getUnknownExplanation? then .unknown unkTxt.toString
+  else .other s!"could not extract any information from cvc5 result"
+
+/-- String representation. -/
+protected def toString : CheckSat → String
+| sat => "sat"
+| unsat => "unsat"
+| unknown msg => s!"unknown[{msg}]"
+| other msg => s!"?[{msg}]?"
+
+instance : ToString CheckSat := ⟨CheckSat.toString⟩
+
+end CheckSat
