Cvc/Basic/Batteries.lean
@@ -1,0 +1,210 @@
+/-
+Copyright (c) 2025 by the authors listed in the file AUTHORS and their
+institutional affiliations. All rights reserved.
+Released under Apache 2.0 license as described in the file LICENSE.
+Authors: Adrien Champion
+-/
+
+import Batteries.Data.HashMap.Basic
+import Batteries.Data.RBMap
+
+import Cvc.Basic.Basic
+
+
+
+/-! # Re-exports from `Batteries` -/
+namespace Cvc
+
+
+
+/-! ## `RBMap` -/
+
+@[inherit_doc Batteries.RBMap]
+abbrev RBMap (α β : Type) [Ord α] :=
+  Batteries.RBMap α β compare
+
+namespace RBMap variable [Ord α]
+
+open Batteries renaming RBMap → Map
+
+/-- The empty map. -/
+def empty : RBMap α β := Map.empty
+
+/-- Builds a map from a list. -/
+def ofList : List (α × β) → RBMap α β :=
+  (Map.ofList · compare)
+
+/-- Removes from `map` the bindings `key`/`val` such that `¬ f key val`. -/
+def filter : (map : RBMap α β) → (f : α → β → Bool) → RBMap α β :=
+  Map.filter
+
+/-- Removes from `map` the bindings `key`/`val` such that `¬ f val`. -/
+def filterVal (map : RBMap α β) (f : β → Bool) : RBMap α β :=
+  map.filter fun _ => f
+
+/-- Inserts a `key`/`val` binding in a map.
+
+See also `RBMap.insert'`.
+-/
+def insert : (map : RBMap α β) → (key : α) → (val : β) → RBMap α β :=
+  Map.insert
+
+/-- Adds a `key`/`val` binding in a map, returns the previous value of `key` if any.
+
+See also `RBMap.insert`.
+-/
+def insert' (map : RBMap α β) (key : α) (val : β) : (Option β) × RBMap α β :=
+  (map.find? key, map.insert key val)
+
+/-- Adds a `key`/`val` binding in a map, `none` if a binding for `key` already exists. -/
+def insertNew? (map : RBMap α β) (key : α) (val : β) : Option (RBMap α β) :=
+  let (prev?, map) := map.insert' key val
+  prev?.map (𝕂 map)
+
+/-- Removes from `map` the binding for `key`, if any.
+
+See also `RBMap.erase'`.
+-/
+def erase : (map : RBMap α β) → (key : α) → RBMap α β :=
+  Map.erase
+
+/-- Removes a `key`/`val` binding from a map, yields `some val` if such a binding existed.
+
+See also `RBMap.erase`.
+-/
+def erase' (map : RBMap α β) (key : α) : (Option β) × RBMap α β :=
+  (map.find? key, map.erase key)
+
+/-- Removes a `key`/`val` binding from a map, `none` if no binding for `key` existed. -/
+def eraseExisting? (map : RBMap α β) (key : α) : Option (RBMap α β) :=
+  match map.erase' key with
+  | (some _, map) => map
+  | (none, _) => none
+
+/-- Map over the values of a map. -/
+def mapVal : (f : α → β → γ) → (map : RBMap α β) → RBMap α γ :=
+  Map.mapVal
+
+/-- Monadic filter/map over the values of a map. -/
+def filterMapValM [Monad m] (f : α → β → m (Option γ)) (map : RBMap α β) : m (RBMap α γ) :=
+  RBMap.empty |> map.foldlM fun map key val => do
+    if let some val ← f key val then return map.insert key val else return map
+
+/-- Monadic map over the values of a map. -/
+def mapValM [Monad m] (f : α → β → m γ) (map : RBMap α β) : m (RBMap α γ) :=
+  map.filterMapValM (some <$> f · ·)
+
+/-- Filter/map over the values of a map. -/
+def filterMapVal (f : α → β → Option γ) (map : RBMap α β) : RBMap α γ :=
+  map.filterMapValM (m := Id) f
+
+/-- Monadic filter/map over the values of a map into an array of values. -/
+def filterMapValToArrayM [Monad m] (f : α → β → m (Option γ)) (map : RBMap α β) : m (Array γ) :=
+  #[] |> map.foldlM fun array key val => do
+    if let some val ← f key val then return array.push val else return array
+
+/-- Filter/map over the values of a map into an array of values. -/
+def filterMapValToArray (f : α → β → Option γ) (map : RBMap α β) : Array γ :=
+  map.filterMapValToArrayM (m := Id) f
+
+/-- Monadic map over the values of a map into an array of values. -/
+def mapValToArrayM [Monad m] (f : α → β → m γ) (map : RBMap α β) : m (Array γ) :=
+  map.filterMapValToArrayM (some <$> f · ·)
+
+/-- Map over the values of a map into an array of values. -/
+def mapValToArray (f : α → β → γ) (map : RBMap α β) : Array γ :=
+  map.mapValToArrayM (m := Id) f
+
+/-- Monadic key-ignoring map over the values of a map. -/
+def mapOnlyValM [Monad m] (f : β → m γ) (map : RBMap α β) : m (RBMap α γ) :=
+  map.mapValM fun _ => f
+
+/-- Key-ignoring map over the values of a map. -/
+def mapOnlyVal (f : β → γ) (map : RBMap α β) : RBMap α γ :=
+  map.mapVal fun _ => f
+
+/-- Key-ignoring monadic filter/map over the values of a map. -/
+def filterMapOnlyValM [Monad m] (f : β → m (Option γ)) (map : RBMap α β) : m (RBMap α γ) :=
+  map.filterMapValM fun _ => f
+
+/-- Key-ignoring filter/map over the values of a map. -/
+def filterMapOnlyVal (f : β → Option γ) (map : RBMap α β) : RBMap α γ :=
+  map.filterMapOnlyValM (m := Id) f
+
+/-- Key-ignoring filter/map over the values of a map into an array of values. -/
+def filterMapOnlyValToArrayM [Monad m] (f : β → m (Option γ)) (map : RBMap α β) : m (Array γ) :=
+  map.filterMapValToArrayM fun _ => f
+
+/-- Key-ignoring filter/map over the values of a map into an array of values. -/
+def filterMapOnlyValToArray (f : β → Option γ) (map : RBMap α β) : Array γ :=
+  map.filterMapOnlyValToArrayM (m := Id) f
+
+/-- Key-ignoring monadic map over the values of a map into an array of values. -/
+def mapOnlyValToArrayM [Monad m] (f : β → m γ) (map : RBMap α β) : m (Array γ) :=
+  map.mapValToArrayM fun _ => f
+
+/-- Key-ignoring map over the values of a map into an array of values. -/
+def mapOnlyValToArray (f : β → γ) (map : RBMap α β) : Array γ :=
+  map.mapOnlyValToArrayM (m := Id) f
+
+def filterMapFoldM {Acc : Type} [Monad m] (init : Acc)
+  (f : Acc → α → β → m (Acc × Option γ))
+  (map : RBMap α β)
+: m (Acc × RBMap α γ) := do
+  let mut map' : RBMap α γ := .empty
+  let mut acc := init
+  for (key, val) in map do
+    let (acc', val?) ← f acc key val
+    acc := acc'
+    if let some val := val? then
+      map' := map'.insert key val
+  return (acc, map')
+
+
+end RBMap
+
+
+
+@[inherit_doc Batteries.RBSet]
+abbrev RBSet (α : Type) [Ord α] :=
+  Batteries.RBSet α compare
+
+namespace RBSet variable [Ord α]
+
+open Batteries renaming RBSet → Set
+
+/-- The empty set. -/
+def empty : RBSet α := Set.empty
+
+/-- Removes from `set` the elements `elm` for which `¬ f elm`. -/
+def filter : (set : RBSet α) → (f : α → Bool) → RBSet α :=
+  Set.filter
+
+/-- Inserts an element in the set.
+
+See also `RBSet.insert'`.
+-/
+def insert : (set : RBSet α) → α → RBSet α :=
+  Set.insert
+
+/-- Inserts an element in the set, yields `true` *iff* the element is new.
+
+See also `RBSet.insert`.
+-/
+def insert' (set : RBSet α) (elm : α) : Bool × RBSet α :=
+  (set.contains elm, set.insert elm)
+
+/-- Removes an element from a set.
+
+See also `RBSet.erase'`.
+-/
+def erase (set : RBSet α) (k : α) : RBSet α := Set.erase set (compare k)
+
+/-- Removes an element from a set, yields `true` *iff* the element was there.
+
+See also `RBSet.erase`
+-/
+def erase' (set : RBSet α) (elm : α) : Bool × RBSet α :=
+  (set.contains elm, set.insert elm)
+
+end RBSet
