Cvc/Basic/Error.lean
@@ -1,0 +1,149 @@
+/-
+Copyright (c) 2025 by the authors listed in the file AUTHORS and their
+institutional affiliations. All rights reserved.
+Released under Apache 2.0 license as described in the file LICENSE.
+Authors: Adrien Champion
+-/
+
+import cvc5
+
+import Cvc.Basic.Basic
+
+
+
+namespace Cvc
+
+
+
+/-- Cvc's error type -/
+inductive Error : Type
+/-- Internal error. -/
+| internal (msg : String)
+/-- Unsupported feature. -/
+| unsupported (msg : String)
+/-- User-input error. -/
+| user (msg : String)
+/-- Input/output error. -/
+| io (msg : String)
+deriving Inhabited
+
+
+namespace Error
+
+/-- Used to allow `String` and `Unit → String` as context messages. -/
+class AsString (α : Type) : Type where
+  /-- Conversion to strings. -/
+  asString : α → String
+
+instance : AsString String := ⟨id⟩
+instance : AsString (Unit → String) := ⟨fun f => f ()⟩
+
+/-- Map over an error's internal message -/
+def mapMsg (f : String → String) : Error → Error
+| .internal msg => f msg |> .internal
+| .unsupported msg => f msg |> .unsupported
+| .user msg => f msg |> .user
+| .io msg => f msg |> .io
+
+/-- Appends some text to an error's internal message. -/
+def append (self : Error) (txt : String) (newline := true) : Error :=
+  let txt := if newline then "\n"++txt else txt
+  self.mapMsg (· ++ txt)
+
+/-- Conversion to `cvc5` errors. -/
+def toUnsafe : Error → cvc5.Error
+| .internal "a value is missing" => .missingValue
+| .internal msg => .error s!"[internal] {msg}"
+| .unsupported msg => .unsupported msg
+| .user msg => .error msg
+| .io msg => .error s!"[io] {msg}"
+
+/-- Constructor from `cvc5` errors. -/
+def ofUnsafe : cvc5.Error → Error
+| .missingValue => .internal "a value is missing"
+| .error msg => .internal s!"{msg}"
+| .option msg => .internal s!"option error: {msg}"
+| .unsupported msg => .unsupported msg
+| .recoverable msg => .internal s!"recoverable: {msg}"
+
+instance : MonadLift (Except cvc5.Error) (Except Error) where
+  monadLift
+  | .ok res => .ok res
+  | .error e => .error (ofUnsafe e)
+
+instance : Coe cvc5.Error Error := ⟨ofUnsafe⟩
+
+/-- String representation. -/
+protected def toString : Error → String
+| .user msg => msg
+| .internal msg => s!"[internal] {msg}"
+| .unsupported msg => s!"[unsupported] {msg}"
+| .io msg => s!"[io] {msg}"
+
+instance instToString : ToString Error :=
+  ⟨Error.toString⟩
+
+section variable [Monad m] [MonadExcept Error m] (msg : String)
+
+/-- Throws an `Error.user`. -/
+def throwUser : m α := do
+  throw <| Error.user msg
+
+/-- Throws an `Error.internal`. -/
+def throwInternal : m α := do
+  throw <| Error.internal msg
+
+/-- Throws an `Error.internal`. -/
+def throwUnreachable (msg : String := "") : m α := do
+  let sep := if msg.isEmpty then "" else ": "
+  throw <| Error.internal s!"reached unreachable code{sep}{msg}"
+
+/-- Throws an `Error.io`. -/
+def throwIO (e : IO.Error) : m α := do
+  throw <| Error.io <| toString e
+
+end
+
+end Error
+
+export Error (throwUser throwInternal throwUnreachable throwIO)
+
+
+
+/-- Sets an error context as a lazy string to newline-append after `code`'s error, if any. -/
+def errorContext [Monad m] [MonadExcept Error m] (s : Unit → String) (code : m α) : m α :=
+  try code catch e => e.mapMsg (s!"{·}\n{s ()}") |> throw
+
+
+
+/-- `Error`-result monad transformer. -/
+abbrev ResT (m : Type → Type) (α : Type) : Type := ExceptT Error m α
+
+/-- `Error` monad. -/
+abbrev Res (α : Type) : Type := ResT Id α
+
+namespace ResT
+
+-- sanity
+example [Monad m] : Monad (ResT m) := inferInstance
+example [Monad m] : MonadExcept Error (ResT m) := inferInstance
+example [Monad m] : MonadLift m (ResT m) := inferInstance
+
+end ResT
+
+namespace Res
+
+@[inherit_doc Except.ok]
+abbrev ok (a : α) : Res α := return a
+
+@[inherit_doc Except.error]
+abbrev error (e : Error) : Res α := throw e
+
+-- sanity
+example : Monad Res := inferInstance
+example : MonadExcept Error Res := inferInstance
+
+instance [Monad m] : MonadLift Res (ResT m) :=
+  ⟨fun | .ok a => return a | .error e => throw e⟩
+
+end Res
