Cvc/Basic/Srt.lean
@@ -1,0 +1,71 @@
+/-
+Copyright (c) 2025 by the authors listed in the file AUTHORS and their
+institutional affiliations. All rights reserved.
+Released under Apache 2.0 license as described in the file LICENSE.
+Authors: Adrien Champion
+-/
+
+import cvc5
+
+
+
+namespace Cvc
+
+namespace Srt
+
+@[inherit_doc cvc5.SortKind]
+def Kind := cvc5.SortKind
+
+namespace Kind
+
+local syntax "Cvc.Srt.Kind.generatePatterns!" : command
+open Lean Elab Command in
+elab_rules : command
+| `(Cvc.Srt.Kind.generatePatterns!) =>
+  let kindIdent := ``Kind |> mkIdent
+  let array := #[
+    (`null, ``cvc5.SortKind.NULL_SORT),
+    (`abstract, ``cvc5.SortKind.ABSTRACT_SORT),
+    (`array, ``cvc5.SortKind.ARRAY_SORT),
+    (`bag, ``cvc5.SortKind.BAG_SORT),
+    (`boolean, ``cvc5.SortKind.BOOLEAN_SORT),
+    (`bitvector, ``cvc5.SortKind.BITVECTOR_SORT),
+    (`datatype, ``cvc5.SortKind.DATATYPE_SORT),
+    (`finite_field, ``cvc5.SortKind.FINITE_FIELD_SORT),
+    (`floatingpoint, ``cvc5.SortKind.FLOATINGPOINT_SORT),
+    (`function, ``cvc5.SortKind.FUNCTION_SORT),
+    (`integer, ``cvc5.SortKind.INTEGER_SORT),
+    (`real, ``cvc5.SortKind.REAL_SORT),
+    (`reglan, ``cvc5.SortKind.REGLAN_SORT),
+    (`roundingmode, ``cvc5.SortKind.ROUNDINGMODE_SORT),
+    (`sequence, ``cvc5.SortKind.SEQUENCE_SORT),
+    (`set, ``cvc5.SortKind.SET_SORT),
+    (`string, ``cvc5.SortKind.STRING_SORT),
+    (`tuple, ``cvc5.SortKind.TUPLE_SORT),
+    (`nullable, ``cvc5.SortKind.NULLABLE_SORT),
+    (`uninterpreted, ``cvc5.SortKind.UNINTERPRETED_SORT),
+    (`last, ``cvc5.SortKind.LAST_SORT_KIND),
+  ].map fun (n1, n2) => (mkIdent n1, mkIdent n2)
+  for (defIdent, variantIdent) in array do
+    let stx ← `(
+      @[inherit_doc $variantIdent, match_pattern]
+      abbrev $defIdent : $kindIdent := $variantIdent
+    )
+    elabCommand stx
+
+Cvc.Srt.Kind.generatePatterns!
+
+/-- Constructor from an unsafe sort. -/
+def ofUnsafe : cvc5.SortKind → Srt.Kind := id
+
+/-- Conversion to an unsafe sort. -/
+def toUnsafe : Srt.Kind → cvc5.SortKind := id
+
+/-- String representation. -/
+protected def toString : Srt.Kind → String := cvc5.SortKind.toString
+
+instance : ToString Srt.Kind := ⟨Kind.toString⟩
+
+end Kind
+
+end Srt
