Cvc/Ext.lean
@@ -1,12 +1,13 @@
 /-
-Copyright (c) 2023-2025 by the authors listed in the file AUTHORS and their
+Copyright (c) 2025 by the authors listed in the file AUTHORS and their
 institutional affiliations. All rights reserved.
 Released under Apache 2.0 license as described in the file LICENSE.
 Authors: Adrien Champion
 -/
 
+import Lean.Parser
+
 import Cvc.Defs
-import Cvc.Term.Erased
 
 
 
@@ -15,7 +16,7 @@ namespace Cvc.Term.Dsl
 declare_syntax_cat smtTerm
 
 
--- scoped syntax "[|" term "|]" : smtTerm
+
 scoped syntax "![" term "]" : smtTerm
 
 scoped syntax "(" smtTerm ")" : smtTerm
@@ -37,7 +38,7 @@ scoped syntax "⊻[" smtTerm ", " smtTerm (", " smtTerm)* ","? "]" : smtTerm
 scoped syntax:max "¬ " smtTerm:40 : smtTerm
 
 scoped syntax
-  withPosition("if " smtTerm (colGe " then " smtTerm) (colGe " else " (colGt smtTerm)))
+  withPosition("if " smtTerm (colGe " then " smtTerm) (colGe " else " (colGe smtTerm)))
 : smtTerm
 scoped syntax "let " ident " ← " smtTerm "; " ppLine smtTerm : smtTerm
 
@@ -89,79 +90,66 @@ scoped syntax
 end
 
 macro_rules
-| `(smt! fun $[$binders]* $[ : $ty:term ]? => $t:smtTerm ) => `(
-  fun $[$binders]* $[ : $ty ]? => smt! $t
-)
-| `(smt! fun $[$binders]* => $t:smtTerm ) => `(
-  fun $[$binders]* => smt! $t
-)
-| `(smtFun! $[$binders]* $[ : $ty:term ]? => $t:smtTerm ) => `(
-  fun $[$binders]* $[ : $ty:term ]? => smt! $t
-)
-| `(smtFun! $[$binders]* => $t:smtTerm ) => `(
-  fun $[$binders]* => smt! $t
-)
-| `(smtPredicate! $binder:funBinder $[ : $ty:term ]? => $t:smtTerm ) => `(
-  fun $binder:funBinder $[ : $ty:term ]? => smt! $t
-)
-| `(smtPred! $binder:funBinder $[ : $ty:term ]? => $t:smtTerm ) => `(
-  fun $binder:funBinder $[ : $ty:term ]? => smt! $t
-)
-| `(smtRel!
-  $currBinder:funBinder $nextBinder:funBinder $[ : $ty:term ]? => $t:smtTerm
-) => `(
-  fun $currBinder:funBinder $nextBinder:funBinder $[ : $ty:term ]? => smt! $t
-)
-| `(smtRelation!
-  $currBinder:funBinder $nextBinder:funBinder $[ : $ty:term ]? => $t:smtTerm
-) => `(
-  fun $currBinder:funBinder $nextBinder:funBinder $[ : $ty:term ]? => smt! $t
-)
+| `(smt! fun $[$binders]* $[ : $ty:term ]? => $t:smtTerm ) =>
+  `(fun $[$binders]* $[ : $ty ]? => smt! $t)
+| `(smt! fun $[$binders]* => $t:smtTerm ) =>
+  `(fun $[$binders]* => smt! $t)
+| `(smtFun! $[$binders]* $[ : $ty:term ]? => $t:smtTerm ) =>
+  `(fun $[$binders]* $[ : $ty:term ]? => smt! $t)
+| `(smtFun! $[$binders]* => $t:smtTerm ) =>
+  `(fun $[$binders]* => smt! $t)
+| `(smtPredicate! $binder:funBinder $[ : $ty:term ]? => $t:smtTerm ) =>
+  `(fun $binder:funBinder $[ : $ty:term ]? => smt! $t)
+| `(smtPred! $binder:funBinder $[ : $ty:term ]? => $t:smtTerm ) =>
+  `(fun $binder:funBinder $[ : $ty:term ]? => smt! $t)
+| `(smtRel! $currBinder:funBinder $nextBinder:funBinder $[ : $ty:term ]? => $t:smtTerm) =>
+  `(fun $currBinder:funBinder $nextBinder:funBinder $[ : $ty:term ]? => smt! $t)
+| `(smtRelation! $currBinder:funBinder $nextBinder:funBinder $[ : $ty:term ]? => $t:smtTerm) =>
+  `(fun $currBinder:funBinder $nextBinder:funBinder $[ : $ty:term ]? => smt! $t)
 
 -- | `(smt! [| $t:term |]) => `((pure $t))
 | `(smt! ![ $t:term ]) => `($t)
 | `(smt! ($t:smtTerm)) => `(smt! $t)
-| `(smt! ?[ $t:term : $ty:term ]) => `($t >>= fun eTerm => Cvc.ETerm.as eTerm $ty)
+-- | `(smt! ?[ $t:term : $ty:term ]) => ``($t >>= fun eTerm => Cvc.ETerm.as eTerm $ty)
 
-| `(smt! false) => `(Cvc.Term.bool false)
-| `(smt! true) => `(Cvc.Term.bool true)
-| `(smt! $n:ident) => `(pure $n)
-| `(smt! $n:name) => `(pure $n)
-| `(smt! $n:num) => `(Cvc.Term.int $n)
-| `(smt! - $n:num) => `(Cvc.Term.int (- $n))
+| `(smt! false) => ``(Cvc.Term.bool false)
+| `(smt! true) => ``(Cvc.Term.bool true)
+| `(smt! $n:ident) => ``(pure $n)
+| `(smt! $n:name) => ``(pure $n)
+| `(smt! $n:num) => ``(Cvc.Term.int $n)
+| `(smt! - $n:num) => ``(Cvc.Term.int (- $n))
 
 | `(smt! $lft → $rgt) =>
   `( (do Cvc.Term.implies (← smt! $lft) (← smt! $rgt)) )
 | `(smt! →[ $fst:smtTerm, $snd:smtTerm $[ , $tail:smtTerm ]* $[,]? ]) =>
-  `( (do Cvc.Term.mkImplies #[(← smt! ($fst)), (← smt! ($snd)), $[(← smt! ($tail)) ],* ] ) )
+  `( (do Cvc.Term.mkImplies #[(← smt! ($fst)), (← smt! ($snd)), $[(← smt! ($tail)) ],* ]) )
 | `(smt! $lft ∧ $rgt) =>
   `( (do Cvc.Term.and (← smt! $lft) (← smt! $rgt)) )
 | `(smt! ∧[ $fst:smtTerm, $snd:smtTerm $[ , $tail:smtTerm ]* $[,]? ]) =>
-  `( (do Cvc.Term.mkAnd #[(← smt! ($fst)), (← smt! ($snd)), $[(← smt! ($tail)) ],* ] ) )
+  `( (do Cvc.Term.mkAnd #[(← smt! ($fst)), (← smt! ($snd)), $[(← smt! ($tail)) ],* ]) )
 | `(smt! $lft ∨ $rgt) =>
   `( (do Cvc.Term.or (← smt! $lft) (← smt! $rgt)) )
 | `(smt! ∨[ $fst:smtTerm, $snd:smtTerm $[ , $tail:smtTerm ]* $[,]? ]) =>
-  `( (do Cvc.Term.mkOr #[(← smt! ($fst)), (← smt! ($snd)), $[(← smt! ($tail)) ],* ] ) )
+  `( (do Cvc.Term.mkOr #[(← smt! ($fst)), (← smt! ($snd)), $[(← smt! ($tail)) ],* ]) )
 | `(smt! $lft ⊻ $rgt) =>
   `( (do Cvc.Term.xor (← smt! $lft) (← smt! $rgt)) )
 | `(smt! ⊻[ $fst:smtTerm, $snd:smtTerm $[ , $tail:smtTerm ]* $[,]? ]) =>
-  `( (do Cvc.Term.mkXor #[(← smt! ($fst)), (← smt! ($snd)), $[(← smt! ($tail)) ],* ] ) )
+  `( (do Cvc.Term.mkXor #[(← smt! ($fst)), (← smt! ($snd)), $[(← smt! ($tail)) ],* ]) )
 | `(smt! ¬ $t) =>
   `( (do Cvc.Term.not (← smt! $t)) )
 
 | `(smt! if $cnd then $thn else $els) =>
   `( (do Cvc.Term.ite (← smt! $cnd) (← smt! $thn) (← smt! $els)) )
 
-| `(smt! let $id ← $idDef ; $tail) =>
-  `( (do
-        let $id ← smt! $idDef
-        smt! $tail
-  ) )
+| `(smt! let $id ← $idDef ; $tail) => `( ( do
+  let $id ← smt! $idDef
+  smt! $tail
+) )
 
 | `(smt! $lft = $rgt) =>
-  `( (do Cvc.Term.equal (← smt! $lft) (← smt! $rgt)) )
+  `( (do Cvc.Term.eq (← smt! $lft) (← smt! $rgt)) )
 | `(smt! =[ $fst:smtTerm, $snd:smtTerm $[ , $tail:smtTerm ]* $[,]? ]) =>
-  `( (do Cvc.Term.mkEqual #[(← smt! ($fst)), (← smt! ($snd)), $[(← smt! ($tail)) ],* ] ) )
+  `( (do Cvc.Term.mkEq #[(← smt! ($fst)), (← smt! ($snd)), $[(← smt! ($tail)) ],* ]) )
 | `(smt! $lft ≠ $rgt) =>
   `( (do Term.distinct (← smt! $lft) (← smt! $rgt)) )
 | `(smt! ≠[ $fst:smtTerm, $snd:smtTerm $[ , $tail:smtTerm ]* $[,]? ]) =>
@@ -184,9 +172,7 @@ macro_rules
   `( (do Cvc.Term.mkGt #[(← smt! ($fst)), (← smt! ($snd)), $[(← smt! ($tail)) ],* ]) )
 
 | `(smt! $f:smtTerm $arg:smtTerm) =>
-  `( (do
-    Term.apply (← smt! $f) (← smt! $arg)
-  ) )
+  `( (do Term.apply (← smt! $f) (← smt! $arg)) )
 
 | `(smt! $lft * $rgt) =>
   `( (do Cvc.Term.mul (← smt! $lft) (← smt! $rgt)) )
