Cvc/Symbols.lean
@@ -1,11 +1,64 @@
 /-
-Copyright (c) 2023-2025 by the authors listed in the file AUTHORS and their
+Copyright (c) 2025 by the authors listed in the file AUTHORS and their
 institutional affiliations. All rights reserved.
 Released under Apache 2.0 license as described in the file LICENSE.
 Authors: Adrien Champion
 -/
 
-import Cvc.Symbols.Basic
-import Cvc.Symbols.Defs
-import Cvc.Symbols.Dsl
-import Cvc.Symbols.Erased
+import Cvc.Defs
+
+
+
+namespace Cvc
+
+
+
+structure Symbol [Cvc.Scope] (α : Type) where
+  get : α
+  sort : Srt
+
+
+namespace Symbol variable [Cvc.Scope]
+
+instance : Coe (Symbol α) α := ⟨get⟩
+
+def Ident := Symbol String
+
+def Term := Symbol Cvc.Term
+
+/-- The `Cvc.Term` in a `Term`. -/
+def toTerm (symbol : Term) : Cvc.Term := symbol.get
+
+def Val := Symbol Cvc.Term
+
+structure TermAt (k : Nat) extends Term where
+private mk' ::
+
+structure ValAt (k : Nat) extends Val
+
+def declare (symbol : Ident) : Env Term :=
+  return { symbol with get := ← Term.symbol symbol.get symbol.sort }
+
+def declareAt (symbol : Ident) (k : Nat) : Env (TermAt k) := do
+  let ident := s!"{symbol.get}__@__{k}"
+  return { get := ← Term.symbol ident symbol.sort, sort := symbol.sort }
+
+def getValue (symbol : Term) (solver : Solver) : Env.Sat Val :=
+  return { symbol with get := ← solver.getValue symbol.get }
+
+namespace TermAt variable (symbol : TermAt k)
+
+def mk (symbol : String) (k : Nat) (sort : Srt) : Env (TermAt k) := do
+  declareAt ⟨symbol, sort⟩ k
+
+/-- The `Cvc.Term` in a `TermAt _`. -/
+def toTerm : Cvc.Term := symbol.get
+
+instance : CoeDep (TermAt k) symbol Cvc.Term := ⟨symbol.toTerm⟩
+
+def getValue (solver : Solver) : Env.Sat (ValAt k) := do
+  return ⟨← Symbol.getValue symbol.toSymbol solver⟩
+
+end TermAt
+
+end Symbol
