Tests/Demo/Induction.lean
@@ -1,0 +1,373 @@
+/-
+Copyright (c) 2025 by the authors listed in the file AUTHORS and their
+institutional affiliations. All rights reserved.
+Released under Apache 2.0 license as described in the file LICENSE.
+Authors: Adrien Champion
+-/
+
+import Cvc
+
+
+
+namespace Cvc.Induction variable [Cvc.Scope]
+
+
+
+inductive Typ
+| bool
+| int
+| real
+| string
+
+namespace Typ
+
+protected def toString : Typ → String
+| bool => "bool"
+| int => "int"
+| real => "real"
+| string => "string"
+
+instance : ToString Typ := ⟨Typ.toString⟩
+
+def toSort : Typ → Env Srt
+| bool => Srt.bool
+| int => Srt.int
+| real => Srt.real
+| string => Srt.string
+
+end Typ
+
+
+
+class State (S : Type → Type) where
+  mapM {m : Type → Type} {α β : Type} : [Monad m] → S α → (α → Typ → m β) → m (S β)
+  foldM {m : Type → Type} {α σ : Type} : [Monad m] → S α → (σ → α → Typ → m σ) → σ → m σ
+
+namespace State variable [σ : State S]
+
+def iterM {m : Type → Type} [Monad m] (state : S α) (f : α → Typ → m Unit) : m Unit :=
+  σ.foldM state (fun _ => f) ()
+
+protected abbrev Idents [State S] : Type := S String
+
+protected abbrev At [State S] (k : Nat) : Type := S (Symbol.TermAt k)
+
+protected abbrev ValAt [State S] (k : Nat) : Type := S (Symbol.ValAt k)
+
+abbrev Pred : Type := {k : Nat} → (state : σ.At k) → Env Term
+
+abbrev Rel : Type := {k k' : Nat} → (prev : σ.At k) → (curr : σ.At k') → Env Term
+
+abbrev Candidates : Type := Array (σ.Pred × String)
+
+def declareAt (k : Nat) (idents : σ.Idents) : Env (σ.At k) :=
+  σ.mapM idents fun ident type => type.toSort >>= Symbol.TermAt.mk ident k
+
+def declareAbstract (idents : σ.Idents) : Env (S Term) :=
+  σ.mapM idents fun ident type => type.toSort >>= Term.symbol ident
+
+def getValues (state : σ.At k) (solver : Solver) : Env.Sat (σ.ValAt k) :=
+  σ.mapM state fun term _ => term.getValue solver
+
+abbrev ValsAt (k : Nat) : Type := S (Symbol.ValAt k)
+
+inductive Trace? (F : Nat → Type) : Nat → Type
+| zero : F 0 → Trace? F 0
+| succ : F k.succ → Trace? F k → Trace? F k.succ
+
+abbrev Trace k := Trace? σ.At k
+
+abbrev Cex k := Trace? σ.ValAt k
+
+namespace Trace?
+
+def len (_ : Trace? F k) := k
+
+def highest : Trace? F k → F k
+| zero f => f
+| succ f _ => f
+
+def atZero : Trace? F k → F 0
+| zero f => f
+| succ _ tail => tail.atZero
+
+def getCex (solver : Solver) : σ.Trace k → Env.Sat (σ.Cex k)
+| zero f0 => zero <$> σ.getValues f0 solver
+| succ fk tail => do
+  let fk ← σ.getValues fk solver
+  succ fk <$> tail.getCex solver
+
+end Trace?
+
+structure Sys [σ : State S] where
+  state : σ.Idents
+  base : σ.Pred
+  step : σ.Rel
+  candidates : σ.Candidates
+
+namespace Sys
+
+/-- A candidate index. -/
+abbrev Idx (spec : σ.Sys) := Fin spec.candidates.size
+
+end Sys
+
+end State
+
+
+
+namespace Sys
+
+section variable [σ : State S] (spec : σ.Sys)
+
+inductive Status
+| valid (k : Nat) (strength : RBSet spec.Idx)
+| invalid (cex : σ.Cex k) (also : RBSet spec.Idx)
+| unknown
+
+namespace Status
+
+def isUnknown : Status spec → Bool
+| unknown => true
+| valid _ _ | invalid  _ _ => false
+
+def isValid : Status spec → Bool
+| valid _ _ => true
+| unknown | invalid  _ _ => false
+
+def isInvalid : Status spec → Bool
+| invalid _ _ => true
+| unknown | valid  _ _ => false
+
+end Status
+
+structure Candidate where
+private mk' ::
+  idx : spec.Idx
+  stepPos : Term
+  stepNeg : Term
+  status : Status spec
+
+abbrev Candidates := Array (Candidate spec)
+
+namespace Candidates variable {spec} variable (cs : Candidates spec)
+
+def mapUnknownM [Monad m] (f : Candidate spec → m (Candidate spec)) : m (Candidates spec) :=
+  cs.mapM fun c => if c.status.isUnknown then f c else return c
+
+def filterMapUnknown (f : Candidate spec → α) : Array α :=
+  cs.filterMap fun c => if c.status.isUnknown then f c else none
+
+def filterUnknown : Array (Candidate spec) := cs.filterMapUnknown id
+
+def filterMapValid (f : Candidate spec → α) : Array α :=
+  cs.filterMap fun c => if c.status.isValid then f c else none
+
+def filterValid : Array (Candidate spec) := cs.filterMapValid id
+
+def filterMapInvalid (f : Candidate spec → α) : Array α :=
+  cs.filterMap fun c => if c.status.isInvalid then f c else none
+
+def filterInvalid : Array (Candidate spec) := cs.filterMapInvalid id
+
+end Candidates
+
+end
+
+end Sys
+
+
+
+structure Sys (S : Type → Type) [σ : State S]
+extends toSpec : σ.Sys where private mk' ::
+  abstractState : S Term
+  baseSolver : Solver
+  stepSolver : Solver
+  candidates' : Sys.Candidates toSpec
+  k : Nat
+  trace : σ.Trace k
+
+namespace Sys variable [σ : State S]
+
+def mkActlit (desc : String) : Env Term :=
+  Term.boolSymbol s!"_actlit_candidate_{desc}_"
+
+def mkActlitFor {spec : σ.Sys} (candidateIdx : spec.Idx) (desc : String) : Env Term :=
+  mkActlit s!"{candidateIdx}_{desc}"
+
+namespace Candidate
+
+def mk {spec : σ.Sys} (idx : spec.Idx) : Env (Candidate spec) := do
+  let stepPos ← mkActlitFor idx "step_positive"
+  let stepNeg ← mkActlitFor idx "step_negative"
+  return ⟨idx, stepPos, stepNeg, .unknown⟩
+
+end Candidate
+
+namespace Candidates
+
+def mk (spec : σ.Sys) : Env (Candidates spec) := do
+  spec.candidates.mapFinIdxM fun idx _ h => Candidate.mk ⟨idx, h⟩
+
+end Candidates
+
+def mk (spec : σ.Sys) : Env (Sys S) := do
+  let candidates ← Candidates.mk spec
+  let abstractState ← σ.declareAbstract spec.state
+  let at0 ← σ.declareAt 0 spec.state
+  let baseSolver ← Solver.mk "induction base solver" true
+  baseSolver.setOption "produce-models" "true"
+  baseSolver.setOption "produce-unsat-cores" "true"
+  spec.base at0 >>= baseSolver.assert
+  let stepSolver ← Solver.mk "induction reverse-step solver" true
+  stepSolver.setOption "produce-models" "true"
+  stepSolver.setOption "produce-unsat-cores" "true"
+  for candidate in candidates do
+    spec.candidates[candidate.idx].fst at0
+    >>= Term.not
+    >>= stepSolver.activeAssert (act := candidate.stepNeg)
+  return ⟨spec, abstractState, baseSolver, stepSolver, candidates, 0, .zero at0⟩
+
+section variable (sys : Sys S)
+
+def isDone : Bool :=
+  ¬ sys.candidates'.any fun c => c.status.isUnknown
+
+abbrev Idx := sys.toSpec.Idx
+
+def candidatePred (idx : sys.Idx) : σ.Pred := sys.candidates[idx].fst
+def candidateDesc (idx : sys.Idx) : String := sys.candidates[idx].snd
+
+def print (sys : Sys S) (pref : String := "") (withState : Bool := false) : Env Unit := do
+  if withState then
+    println! "{pref}state"
+    σ.iterM sys.abstractState fun (symbol : Term) typ => do
+      println! "{pref}- {← symbol.toSmtString} | {typ}"
+  println! "{pref}candidates"
+  for c in sys.candidates' do
+    match c.status with
+    | .unknown => println! "{pref}-[{c.idx}]-[unknown] \"{sys.candidateDesc c.idx}\""
+    | .valid k set => do
+      println! "{pref}-[{c.idx}]-[valid@{k}] \"{sys.candidateDesc c.idx}\""
+      if 1 < set.size then println! "{pref}    proved in cluster {set.toList}"
+    | .invalid trace set => do
+      println! "{pref}-[{c.idx}]-[invalid@{trace.len}] \"{sys.candidateDesc c.idx}\""
+      if 1 < set.size then println! "{pref}    falsified in cluster {set.toList}"
+
+def unroll : Env ((sys' : Sys S) ×' sys'.k = sys.k + 1) := do
+  let atK := sys.trace.highest
+  let atNextK ← σ.declareAt sys.k.succ sys.toSpec.state
+  let trace : σ.Trace sys.k.succ := sys.trace.succ atNextK
+  -- base: unroll forward
+  let step ← sys.step atK atNextK
+  sys.baseSolver.assert step
+  -- step: unroll backward
+  let step ← sys.step atNextK atK
+  sys.stepSolver.assert step
+  -- step actlits
+  for c in sys.candidates'.filterUnknown do
+    let pred ← sys.candidatePred c.idx atNextK
+    sys.stepSolver.activeAssert c.stepPos pred
+  return ⟨{sys with k := sys.k.succ, trace}, rfl⟩
+
+def checkBase' : Env ((sys' : Sys S) ×' sys'.k = sys.k + 1) := do
+  let ⟨sys', h_sys'⟩ ← loop sys sys.candidates'.size.succ
+  h_sys' ▸ sys'.unroll
+where
+  loop (sys : Sys S) : Nat → Env ((sys' : Sys S) ×' sys'.k = sys.k)
+  | 0 => throwInternal s!"[checkBase] maximal number of iterations reached"
+  | n + 1 => do
+    let solver := sys.baseSolver
+    -- sanity, make sure base solver is sat
+    let res ← solver.checkSat?
+    if res.isSat? ≠ some true then
+      throwInternal s!"illegal base solver state, expected `sat` but got `{res}`"
+    let unknown := sys.candidates'.filterUnknown
+    let state := sys.trace.highest
+    let mut anyBadCandidate ← Term.bool false
+    for candidate in unknown do
+      let pred ← sys.candidatePred candidate.idx state
+      anyBadCandidate ← pred.not >>= anyBadCandidate.or
+    solver.checkSat #[anyBadCandidate]
+      (ifUnsat := return ⟨sys, rfl⟩)
+      (ifSat := do
+        let cex ← sys.trace.getCex solver
+        let falsified : RBSet sys.Idx ←
+          unknown.foldlM (init := RBSet.empty) fun set candidate => do
+            let pred ← sys.candidatePred candidate.idx state
+            let isValid ← solver.getValue pred >>= Term.boolVal
+            return if isValid then set else set.insert candidate.idx
+        let candidates' := sys.candidates'.mapUnknownM (m := Id)
+          fun candidate =>
+            if candidate.idx ∈ falsified
+            then {candidate with status := .invalid cex falsified}
+            else candidate
+        let sys := {sys with candidates'}
+        if sys.isDone then return ⟨sys, rfl⟩ else loop sys n)
+
+def checkBase : Env (Sys S) := PSigma.fst <$> sys.checkBase'
+
+def checkStep'
+: (valid : 0 < sys.k := by (try simp) <;> grind)
+→ Env ((sys' : Sys S) ×' sys'.k = sys.k) :=
+  fun _ => loop sys sys.candidates'.filterUnknown sys.candidates'.size.succ
+where
+  checkIsSat (solver : Solver) (desc : String) : Env Unit := do
+    solver.logComment fun () => s!"sanity, make sure step solver is sat - {desc}"
+    if let some core ← solver.checkUnsatCore? then
+      let msg ←
+        s!"illegal step solver state ({desc}), expected `sat` but got `unsat`\nunsat core:"
+        |> core.foldlM (return s!"{·}\n- {← Term.toSmtString ·}")
+      throwInternal msg
+  loop (sys : Sys S) (unknown : Candidates sys.toSpec)
+  : Nat → Env ((sys' : Sys S) ×' sys'.k = sys.k)
+  | 0 => throwInternal s!"[checkStep] maximal number of iterations reached"
+  | n + 1 => do
+    let solver := sys.stepSolver
+    checkIsSat solver "unrolling only"
+    let mut actlits := #[]
+    let mut anyBadCandidate ← Term.bool false
+    for candidate in unknown do
+      anyBadCandidate ← anyBadCandidate.or candidate.stepNeg
+      actlits := actlits ++ #[candidate.stepPos]
+    checkIsSat solver "unrolling and positive actlits"
+    solver.checkSat (actlits.push anyBadCandidate)
+      (ifSat := do
+        let state := sys.trace.atZero
+        let unknown ← unknown.filterM
+          fun c => do
+            let pred ← sys.candidatePred c.idx state
+            solver.getValue pred >>= Term.boolVal
+        if unknown.isEmpty then return ⟨sys, rfl⟩ else loop sys unknown n)
+      (ifUnsat := do
+        let validSet := RBSet.empty |> unknown.foldl fun set c => set.insert c.idx
+        let candidates' ← sys.candidates'.mapUnknownM fun candidate =>
+          if candidate.idx ∈ validSet
+          then return {candidate with status := .valid sys.k validSet}
+          else return candidate
+        return ⟨{sys with candidates'}, rfl⟩)
+
+def checkStep (valid : 0 < sys.k := by (try simp) <;> grind) : Env (Sys S) :=
+  PSigma.fst <$> sys.checkStep' valid
+
+def checkBaseAndStep : Env (Sys S) := do
+  if sys.isDone then return sys
+  let ⟨sys, _⟩ ← sys.checkBase'
+  if sys.isDone then return sys
+  let ⟨sys, _⟩ ← sys.checkStep'
+  return sys
+
+end
+
+def run (sys : Sys S)
+: (n : Nat)
+→ (beforeLoopingDo : Sys S → Env Unit := fun _ => return ())
+→ Env (Sys S)
+| 0, _ => return sys
+| n + 1, beforeLoopingDo => do
+  let sys ← sys.checkBaseAndStep
+  if sys.isDone then return sys
+  beforeLoopingDo sys
+  sys.run n beforeLoopingDo
+
+end Sys
