Tests/Demo/StopWatch.lean
@@ -1,0 +1,178 @@
+/-
+Copyright (c) 2025 by the authors listed in the file AUTHORS and their
+institutional affiliations. All rights reserved.
+Released under Apache 2.0 license as described in the file LICENSE.
+Authors: Adrien Champion
+-/
+
+import Tests.Demo.Induction
+
+
+
+namespace Cvc.Induction.Tests.StopWatch variable [Cvc.Scope]
+
+namespace Sw
+
+protected structure State (α : Type) where
+  startStop : α
+  reset : α
+  counting : α
+  counter : α
+
+def Idents : Sw.State String where
+  startStop := "startStop"
+  reset := "reset"
+  counting := "counting"
+  counter := "counter"
+
+instance Spec : State Sw.State where
+  mapM sw f := return ⟨
+    ← f sw.startStop .bool, ← f sw.reset .bool, ← f sw.counting .bool, ← f sw.counter .int
+  ⟩
+  foldM sw f init := do
+    let mut acc := init
+    acc ← f acc sw.startStop .bool
+    acc ← f acc sw.reset .bool
+    acc ← f acc sw.counting .bool
+    acc ← f acc sw.counter .int
+    return acc
+
+section open scoped Cvc.Term.Dsl
+
+def base : Spec.Pred := fun state =>
+  smt! state.counter = 0 ∧ state.counting = state.startStop
+
+def step : Spec.Rel := fun prev curr => smt!
+  (curr.counting = if curr.startStop then ¬ prev.counting else prev.counting)
+  ∧
+  (curr.counter =
+    if curr.reset then 0 else
+    if curr.counting then prev.counter + 1
+    else prev.counter)
+
+def counter_pos : Spec.Pred × String where
+  fst state := smt! 0 ≤ state.counter
+  snd := "0 ≤ counter"
+
+def counter_not_7 : Spec.Pred × String where
+  fst state := smt! state.counter ≠ 7
+  snd := "counter ≠ 7"
+
+def counter_lt_7 : Spec.Pred × String where
+  fst state := smt! state.counter < 7
+  snd := "counter < 7"
+
+def counter_not_m7 : Spec.Pred × String where
+  fst state := smt! state.counter ≠ -7
+  snd := "counter ≠ -7"
+
+def zero_of_reset : Spec.Pred × String where
+  fst state := smt! state.reset → state.counter = 0
+  snd := "reset → counter = 0"
+
+end
+
+def mk (candidates : Spec.Candidates) : Spec.Sys :=
+  ⟨Sw.Idents, base, step, candidates⟩
+
+def simple : Spec.Sys :=
+  mk #[counter_pos]
+
+def invalid : Spec.Sys :=
+  mk #[counter_not_7]
+
+def unprovable : Spec.Sys :=
+  mk #[counter_not_m7]
+
+def valid := mk #[counter_pos, counter_not_m7, zero_of_reset]
+
+def all := mk #[counter_pos, counter_not_7, counter_lt_7, counter_not_m7, zero_of_reset]
+
+end Sw
+
+def demo (spec : Sw.Spec.Sys)
+  (k : Nat := 1) (stepInfo := false) (showBaseLog := false) (showStepLog := false)
+: Env Unit := do
+  println! "|===| creating system..."
+  let sys ← Sys.mk spec
+  sys.print "| "
+  let sys ← sys.run k
+    (beforeLoopingDo :=
+      if stepInfo then fun sys => do
+        println! "|===| before step {sys.k}"
+        sys.print "| "
+      else fun _ => return ()
+    )
+  if sys.isDone
+  then println! "|===| done after {sys.k} step(s) 🎉"
+  else println! "|===| not done after {sys.k} step(s) 😿"
+  sys.print "| "
+  println! "|===|"
+  if showBaseLog then
+    println! "\nbase solver log:\n```smtlib\n{← sys.baseSolver.getLog}\n```"
+  if showStepLog then
+    println! "\nstep solver log:\n```smtlib\n{← sys.stepSolver.getLog}\n```"
+
+/-- info:
+|===| creating system...
+| candidates
+| -[0]-[unknown] "0 ≤ counter"
+|===| done after 1 step(s) 🎉
+| candidates
+| -[0]-[valid@1] "0 ≤ counter"
+|===|
+-/
+#guard_msgs in #eval Env.runIO <| demo <| Sw.simple
+
+/-- info:
+|===| creating system...
+| candidates
+| -[0]-[unknown] "counter ≠ 7"
+|===| done after 8 step(s) 🎉
+| candidates
+| -[0]-[invalid@7] "counter ≠ 7"
+|===|
+-/
+#guard_msgs in #eval Env.runIO <| demo (k := 10) <| Sw.invalid
+
+/-- info:
+|===| creating system...
+| candidates
+| -[0]-[unknown] "0 ≤ counter"
+| -[1]-[unknown] "counter ≠ -7"
+| -[2]-[unknown] "reset → counter = 0"
+|===| done after 1 step(s) 🎉
+| candidates
+| -[0]-[valid@1] "0 ≤ counter"
+|     proved in cluster [0, 1, 2]
+| -[1]-[valid@1] "counter ≠ -7"
+|     proved in cluster [0, 1, 2]
+| -[2]-[valid@1] "reset → counter = 0"
+|     proved in cluster [0, 1, 2]
+|===|
+-/
+#guard_msgs in #eval Env.runIO <| demo (k := 10) <| Sw.valid
+
+/-- info:
+|===| creating system...
+| candidates
+| -[0]-[unknown] "0 ≤ counter"
+| -[1]-[unknown] "counter ≠ 7"
+| -[2]-[unknown] "counter < 7"
+| -[3]-[unknown] "counter ≠ -7"
+| -[4]-[unknown] "reset → counter = 0"
+|===| done after 8 step(s) 🎉
+| candidates
+| -[0]-[valid@1] "0 ≤ counter"
+|     proved in cluster [0, 3, 4]
+| -[1]-[invalid@7] "counter ≠ 7"
+|     falsified in cluster [1, 2]
+| -[2]-[invalid@7] "counter < 7"
+|     falsified in cluster [1, 2]
+| -[3]-[valid@1] "counter ≠ -7"
+|     proved in cluster [0, 3, 4]
+| -[4]-[valid@1] "reset → counter = 0"
+|     proved in cluster [0, 3, 4]
+|===|
+-/
+#guard_msgs in #eval Env.runIO <| demo (k := 10) <| Sw.all
