Tests/Tmp.lean
@@ -1,0 +1,155 @@
+/-
+Copyright (c) 2025 by the authors listed in the file AUTHORS and their
+institutional affiliations. All rights reserved.
+Released under Apache 2.0 license as described in the file LICENSE.
+Authors: Adrien Champion
+-/
+
+import Cvc.Defs
+import Cvc.Ext
+
+
+
+namespace Cvc.Tests
+
+/-- info:
+- bool := Bool
+- int := Int
+- array := (Array Bool Int)
+- bag := (Bag (Array Bool Int))
+-/
+#guard_msgs in #eval Env.runIO do
+  let bool ← Srt.bool
+  println! "- bool := {←bool.toSmtString}"
+  let int ← Srt.int
+  println! "- int := {←int.toSmtString}"
+  let array ← Srt.array bool int
+  println! "- array := {←array.toSmtString}"
+  let bag ← Srt.bag array
+  println! "- bag := {←bag.toSmtString}"
+
+/-- info:
+- term1 := false
+- term2 := (not false)
+-/
+#guard_msgs in #eval Env.runIO do
+  let term1 ← Term.bool false
+  println! "- term1 := {←term1.toSmtString}"
+  let term2 ← term1.not
+  println! "- term2 := {←term2.toSmtString}"
+
+/-- info:
+- a : Bool := a
+- res := sat
+-/
+#guard_msgs in #eval Env.runIO do
+  let solver ← Solver.mk
+  let bool ← Srt.bool
+  let a ← solver.declareConst "a" bool
+  println! "- a : {←bool.toSmtString} := {←a.toSmtString}"
+  solver.assert a
+  let res ← solver.checkSat?
+  println! "- res := {res}"
+
+/-- info:
+- asserting (ite b1 (not (xor b2 b3)) (or b1 b2 b3))
+- check-sat assuming b2
+- res := sat
+-/
+#guard_msgs in open scoped Term.Dsl in #eval Env.runIO do
+  let solver ← Solver.mk
+  let bool ← Srt.bool
+  let b1 ← solver.declareConst "b1" bool
+  let b2 ← solver.declareConst "b2" bool
+  let b3 ← solver.declareConst "b3" bool
+  let prop ← smt!
+    if b1 then ¬ (b2 ⊻ b3) else ∨[b1, b2, b3]
+  println! "- asserting {← prop.toSmtString}"
+  solver.assert prop
+  println! "- check-sat assuming {← b2.toSmtString}"
+  let res ← solver.checkSat? (assuming := #[b2])
+  println! "- res := {res}"
+
+/--
+info: - asserting (ite (not b1) (not (xor b2 b3)) (or b1 b2 b3))
+- check-sat assuming b2
+- model
+  - b1 ↦ true
+  - b2 ↦ true
+  - b3 ↦ false
+  - irrelevant ↦ 0
+-/
+#guard_msgs in open scoped Term.Dsl in #eval Env.runIO do
+  let solver ← Solver.mk
+  solver.setOption "produce-models" "true"
+  let bool ← Srt.bool
+  let int ← Srt.int
+  let b1 ← solver.declareConst "b1" bool
+  let b2 ← solver.declareConst "b2" bool
+  let b3 ← solver.declareConst "b3" bool
+  let i ← solver.declareConst "irrelevant" int
+  let prop ← smt!
+    if ¬ b1 then ¬ (b2 ⊻ b3) else ∨[b1, b2, b3]
+  println! "- asserting {← prop.toSmtString}"
+  solver.assert prop
+  println! "- check-sat assuming {← b2.toSmtString}"
+  let model ← solver.checkSat (assuming := #[b2])
+    (ifSat := solver.getValueMap #[b1, b2, b3, i])
+  println! "- model"
+  for (term, value) in model do
+    println! "  - {← term.toSmtString} ↦ {← value.toSmtString}"
+
+
+
+
+/-! ## Errors -/
+
+
+
+/--
+error: Application type mismatch: The argument
+  bool
+has type
+  Srt
+but is expected to have type
+  ?m.9
+in the application
+  pure bool
+-/
+#guard_msgs in #eval do
+  let srt ← Env.runIO do
+    let bool ← Srt.bool
+    return bool
+  println! "does not compile"
+
+/--
+error: Application type mismatch: The argument
+  tru
+has type
+  Term
+but is expected to have type
+  ?m.9
+in the application
+  pure tru
+-/
+#guard_msgs in #eval do
+  let term ← Env.runIO do
+    let tru ← Term.bool true
+    return tru
+  println! "does not compile"
+
+/--
+error: Application type mismatch: The argument
+  s
+has type
+  Solver
+but is expected to have type
+  ?m.9
+in the application
+  pure s
+-/
+#guard_msgs in #eval do
+  let solver ← Env.runIO do
+    let s ← Solver.mk
+    return s
+  println! "does not compile"
